Implement rewrite_mov.

src/ocaml/extraction/SSA2SSALite.ml
@@ -1,9 +1,190 @@
+open DSLRaw
+open Datatypes
 open Seqs
+open Typ
+open Var
+
+(** val eexp_of_atom : SSA.SSA.atom -> SSA.SSA.eexp **)
+
+let eexp_of_atom = function
+| Avar v -> SSA.SSA.evar v
+| Aconst (ty, n) -> SSA.SSA.econst (SSA.SSA.bv2z ty n)
+
+(** val rexp_of_atom : SSA.SSA.atom -> SSA.SSA.rexp **)
+
+let rexp_of_atom = function
+| Avar v -> SSA.SSA.rvar v
+| Aconst (ty, n) -> SSA.SSA.rconst (sizeof_typ ty) n
+
+(** val subst_eexp : SSA.SSA.atom SSAVM.t -> SSA.SSA.eexp -> SSA.SSA.eexp **)
+
+let rec subst_eexp m e = match e with
+| Evar v -> (match SSAVM.find v m with
+             | Some a -> eexp_of_atom a
+             | None -> e)
+| Econst _ -> e
+| Eunop (op, e0) -> SSA.SSA.eunary op (subst_eexp m e0)
+| Ebinop (op, e1, e2) ->
+  SSA.SSA.ebinary op (subst_eexp m e1) (subst_eexp m e2)
+| Epow (e0, n) -> SSA.SSA.epow (subst_eexp m e0) n
+
+(** val subst_rexp : SSA.SSA.atom SSAVM.t -> SSA.SSA.rexp -> SSA.SSA.rexp **)
+
+let rec subst_rexp m e = match e with
+| Rvar v -> (match SSAVM.find v m with
+             | Some a -> rexp_of_atom a
+             | None -> e)
+| Rconst (_, _) -> e
+| Runop (w, op, e0) -> SSA.SSA.runary w op (subst_rexp m e0)
+| Rbinop (w, op, e1, e2) ->
+  SSA.SSA.rbinary w op (subst_rexp m e1) (subst_rexp m e2)
+| Ruext (w, e0, i) -> SSA.SSA.ruext w (subst_rexp m e0) i
+| Rsext (w, e0, i) -> SSA.SSA.rsext w (subst_rexp m e0) i
+
+(** val subst_eexps :
+    SSA.SSA.atom SSAVM.t -> SSA.SSA.eexp list -> SSA.SSA.eexp list **)
+
+let subst_eexps m es =
+  tmap (subst_eexp m) es
+
+(** val subst_ebexp :
+    SSA.SSA.atom SSAVM.t -> SSA.SSA.ebexp -> SSA.SSA.ebexp **)
+
+let rec subst_ebexp m e = match e with
+| Etrue -> e
+| Eeq (e1, e2) -> Eeq ((subst_eexp m e1), (subst_eexp m e2))
+| Eeqmod (e1, e2, ms) ->
+  Eeqmod ((subst_eexp m e1), (subst_eexp m e2), (subst_eexps m ms))
+| Eand (e1, e2) -> Eand ((subst_ebexp m e1), (subst_ebexp m e2))
+
+(** val subst_rbexp :
+    SSA.SSA.atom SSAVM.t -> SSA.SSA.rbexp -> SSA.SSA.rbexp **)
+
+let rec subst_rbexp m e = match e with
+| Rtrue -> e
+| Req (w, e1, e2) -> Req (w, (subst_rexp m e1), (subst_rexp m e2))
+| Rcmp (w, op, e1, e2) -> Rcmp (w, op, (subst_rexp m e1), (subst_rexp m e2))
+| Rneg e0 -> Rneg (subst_rbexp m e0)
+| Rand (e1, e2) -> Rand ((subst_rbexp m e1), (subst_rbexp m e2))
+| Ror (e1, e2) -> Ror ((subst_rbexp m e1), (subst_rbexp m e2))
+
+(** val subst_bexp : SSA.SSA.atom SSAVM.t -> SSA.SSA.bexp -> SSA.SSA.bexp **)
+
+let subst_bexp m e =
+  ((subst_ebexp m (fst e)), (subst_rbexp m (snd e)))
+
+(** val subst_atom : SSA.SSA.atom SSAVM.t -> SSA.SSA.atom -> SSA.SSA.atom **)
+
+let subst_atom m a = match a with
+| Avar v -> (match SSAVM.find v m with
+             | Some a' -> a'
+             | None -> a)
+| Aconst (_, _) -> a
+
+(** val subst_instr :
+    SSA.SSA.atom SSAVM.t -> SSA.SSA.instr -> SSA.SSA.instr **)
+
+let subst_instr m i = match i with
+| SSA.SSA.Imov (v, a) -> SSA.SSA.Imov (v, (subst_atom m a))
+| SSA.SSA.Ishl (v, a, n) -> SSA.SSA.Ishl (v, (subst_atom m a), n)
+| SSA.SSA.Icshl (v1, v2, a1, a2, n) ->
+  SSA.SSA.Icshl (v1, v2, (subst_atom m a1), (subst_atom m a2), n)
+| SSA.SSA.Icmov (v, c, a1, a2) ->
+  SSA.SSA.Icmov (v, c, (subst_atom m a1), (subst_atom m a2))
+| SSA.SSA.Inot (v, t0, a) -> SSA.SSA.Inot (v, t0, (subst_atom m a))
+| SSA.SSA.Iadd (v, a1, a2) ->
+  SSA.SSA.Iadd (v, (subst_atom m a1), (subst_atom m a2))
+| SSA.SSA.Iadds (c, v, a1, a2) ->
+  SSA.SSA.Iadds (c, v, (subst_atom m a1), (subst_atom m a2))
+| SSA.SSA.Iadc (v, a1, a2, y) ->
+  SSA.SSA.Iadc (v, (subst_atom m a1), (subst_atom m a2), y)
+| SSA.SSA.Iadcs (c, v, a1, a2, y) ->
+  SSA.SSA.Iadcs (c, v, (subst_atom m a1), (subst_atom m a2), y)
+| SSA.SSA.Isub (v, a1, a2) ->
+  SSA.SSA.Isub (v, (subst_atom m a1), (subst_atom m a2))
+| SSA.SSA.Isubc (c, v, a1, a2) ->
+  SSA.SSA.Isubc (c, v, (subst_atom m a1), (subst_atom m a2))
+| SSA.SSA.Isubb (c, v, a1, a2) ->
+  SSA.SSA.Isubb (c, v, (subst_atom m a1), (subst_atom m a2))
+| SSA.SSA.Isbc (v, a1, a2, y) ->
+  SSA.SSA.Isbc (v, (subst_atom m a1), (subst_atom m a2), y)
+| SSA.SSA.Isbcs (c, v, a1, a2, y) ->
+  SSA.SSA.Isbcs (c, v, (subst_atom m a1), (subst_atom m a2), y)
+| SSA.SSA.Isbb (v, a1, a2, y) ->
+  SSA.SSA.Isbb (v, (subst_atom m a1), (subst_atom m a2), y)
+| SSA.SSA.Isbbs (c, v, a1, a2, y) ->
+  SSA.SSA.Isbbs (c, v, (subst_atom m a1), (subst_atom m a2), y)
+| SSA.SSA.Imul (v, a1, a2) ->
+  SSA.SSA.Imul (v, (subst_atom m a1), (subst_atom m a2))
+| SSA.SSA.Imull (vh, vl, a1, a2) ->
+  SSA.SSA.Imull (vh, vl, (subst_atom m a1), (subst_atom m a2))
+| SSA.SSA.Imulj (v, a1, a2) ->
+  SSA.SSA.Imulj (v, (subst_atom m a1), (subst_atom m a2))
+| SSA.SSA.Isplit (vh, vl, a, n) ->
+  SSA.SSA.Isplit (vh, vl, (subst_atom m a), n)
+| SSA.SSA.Iand (v, t0, a1, a2) ->
+  SSA.SSA.Iand (v, t0, (subst_atom m a1), (subst_atom m a2))
+| SSA.SSA.Ior (v, t0, a1, a2) ->
+  SSA.SSA.Ior (v, t0, (subst_atom m a1), (subst_atom m a2))
+| SSA.SSA.Ixor (v, t0, a1, a2) ->
+  SSA.SSA.Ixor (v, t0, (subst_atom m a1), (subst_atom m a2))
+| SSA.SSA.Icast (v, t0, a) -> SSA.SSA.Icast (v, t0, (subst_atom m a))
+| SSA.SSA.Ivpc (v, t0, a) -> SSA.SSA.Ivpc (v, t0, (subst_atom m a))
+| SSA.SSA.Ijoin (v, ah, al) ->
+  SSA.SSA.Ijoin (v, (subst_atom m ah), (subst_atom m al))
+| SSA.SSA.Icut e -> SSA.SSA.Icut (subst_bexp m e)
+| SSA.SSA.Iassert e -> SSA.SSA.Iassert (subst_bexp m e)
+| SSA.SSA.Iassume e -> SSA.SSA.Iassume (subst_bexp m e)
+| _ -> i
+
+(** val subst_program :
+    SSA.SSA.atom SSAVM.t -> SSA.SSA.program -> SSA.SSA.program **)
+
+let subst_program m p =
+  tmap (subst_instr m) p
+
+(** val subst_spec : SSA.SSA.atom SSAVM.t -> SSA.SSA.spec -> SSA.SSA.spec **)
+
+let subst_spec m s =
+  { SSA.SSA.sinputs = (SSA.SSA.sinputs s); SSA.SSA.spre =
+    (subst_bexp m (SSA.SSA.spre s)); SSA.SSA.sprog =
+    (subst_program m (SSA.SSA.sprog s)); SSA.SSA.spost =
+    (subst_bexp m (SSA.SSA.spost s)) }
+
+(** val subst_map_instr :
+    SSA.SSA.atom SSAVM.t -> SSA.SSA.instr -> SSA.SSA.atom SSAVM.t **)
+
+let subst_map_instr m = function
+| SSA.SSA.Imov (v, a) ->
+  (match a with
+   | Avar u ->
+     (match SSAVM.find u m with
+      | Some ua -> SSAVM.add v ua m
+      | None -> SSAVM.add v a m)
+   | Aconst (_, _) -> SSAVM.add v a m)
+| _ -> m
+
+(** val subst_map_program_rec :
+    SSA.SSA.atom SSAVM.t -> SSA.SSA.program -> SSA.SSA.atom SSAVM.t **)
+
+let rec subst_map_program_rec m = function
+| [] -> m
+| i :: p0 -> subst_map_program_rec (subst_map_instr m i) p0
+
+(** val subst_map_program : SSA.SSA.program -> SSA.SSA.atom SSAVM.t **)
+
+let subst_map_program p =
+  subst_map_program_rec SSAVM.empty p
+
+(** val subst_map_spec : SSA.SSA.spec -> SSA.SSA.atom SSAVM.t **)
+
+let subst_map_spec s =
+  subst_map_program (SSA.SSA.sprog s)
 
 (** val rewrite_mov : SSA.SSA.spec -> SSA.SSA.spec **)
 
 let rewrite_mov s =
-  s
+  subst_spec (subst_map_spec s) s
 
 (** val ssa2lite_instr : SSA.SSA.instr -> SSALite.SSALite.instr **)
 
@@ -12,9 +193,9 @@ let ssa2lite_instr = function
 | SSA.SSA.Ishl (v, a, n) -> SSALite.SSALite.Ishl (v, a, n)
 | SSA.SSA.Icshl (v1, v2, a1, a2, n) ->
   SSALite.SSALite.Icshl (v1, v2, a1, a2, n)
-| SSA.SSA.Inondet (v, t) -> SSALite.SSALite.Inondet (v, t)
+| SSA.SSA.Inondet (v, t0) -> SSALite.SSALite.Inondet (v, t0)
 | SSA.SSA.Icmov (v, c, a1, a2) -> SSALite.SSALite.Icmov (v, c, a1, a2)
-| SSA.SSA.Inot (v, t, a) -> SSALite.SSALite.Inot (v, t, a)
+| SSA.SSA.Inot (v, t0, a) -> SSALite.SSALite.Inot (v, t0, a)
 | SSA.SSA.Iadd (v, a1, a2) -> SSALite.SSALite.Iadd (v, a1, a2)
 | SSA.SSA.Iadds (c, v, a1, a2) -> SSALite.SSALite.Iadds (c, v, a1, a2)
 | SSA.SSA.Iadc (v, a1, a2, y) -> SSALite.SSALite.Iadc (v, a1, a2, y)
@@ -30,11 +211,11 @@ let ssa2lite_instr = function
 | SSA.SSA.Imull (vh, vl, a1, a2) -> SSALite.SSALite.Imull (vh, vl, a1, a2)
 | SSA.SSA.Imulj (v, a1, a2) -> SSALite.SSALite.Imulj (v, a1, a2)
 | SSA.SSA.Isplit (vh, vl, a, n) -> SSALite.SSALite.Isplit (vh, vl, a, n)
-| SSA.SSA.Iand (v, t, a1, a2) -> SSALite.SSALite.Iand (v, t, a1, a2)
-| SSA.SSA.Ior (v, t, a1, a2) -> SSALite.SSALite.Ior (v, t, a1, a2)
-| SSA.SSA.Ixor (v, t, a1, a2) -> SSALite.SSALite.Ixor (v, t, a1, a2)
-| SSA.SSA.Icast (v, t, a) -> SSALite.SSALite.Icast (v, t, a)
-| SSA.SSA.Ivpc (v, t, a) -> SSALite.SSALite.Ivpc (v, t, a)
+| SSA.SSA.Iand (v, t0, a1, a2) -> SSALite.SSALite.Iand (v, t0, a1, a2)
+| SSA.SSA.Ior (v, t0, a1, a2) -> SSALite.SSALite.Ior (v, t0, a1, a2)
+| SSA.SSA.Ixor (v, t0, a1, a2) -> SSALite.SSALite.Ixor (v, t0, a1, a2)
+| SSA.SSA.Icast (v, t0, a) -> SSALite.SSALite.Icast (v, t0, a)
+| SSA.SSA.Ivpc (v, t0, a) -> SSALite.SSALite.Ivpc (v, t0, a)
 | SSA.SSA.Ijoin (v, ah, al) -> SSALite.SSALite.Ijoin (v, ah, al)
 | SSA.SSA.Iassume e -> SSALite.SSALite.Iassume e
 | _ -> SSALite.SSALite.Inop
