src/ocaml/extraction/SSA2SSALite.mli
@@ -1,4 +1,43 @@
+open DSLRaw
+open Datatypes
 open Seqs
+open Typ
+open Var
+
+val eexp_of_atom : SSA.SSA.atom -> SSA.SSA.eexp
+
+val rexp_of_atom : SSA.SSA.atom -> SSA.SSA.rexp
+
+val subst_eexp : SSA.SSA.atom SSAVM.t -> SSA.SSA.eexp -> SSA.SSA.eexp
+
+val subst_rexp : SSA.SSA.atom SSAVM.t -> SSA.SSA.rexp -> SSA.SSA.rexp
+
+val subst_eexps :
+  SSA.SSA.atom SSAVM.t -> SSA.SSA.eexp list -> SSA.SSA.eexp list
+
+val subst_ebexp : SSA.SSA.atom SSAVM.t -> SSA.SSA.ebexp -> SSA.SSA.ebexp
+
+val subst_rbexp : SSA.SSA.atom SSAVM.t -> SSA.SSA.rbexp -> SSA.SSA.rbexp
+
+val subst_bexp : SSA.SSA.atom SSAVM.t -> SSA.SSA.bexp -> SSA.SSA.bexp
+
+val subst_atom : SSA.SSA.atom SSAVM.t -> SSA.SSA.atom -> SSA.SSA.atom
+
+val subst_instr : SSA.SSA.atom SSAVM.t -> SSA.SSA.instr -> SSA.SSA.instr
+
+val subst_program : SSA.SSA.atom SSAVM.t -> SSA.SSA.program -> SSA.SSA.program
+
+val subst_spec : SSA.SSA.atom SSAVM.t -> SSA.SSA.spec -> SSA.SSA.spec
+
+val subst_map_instr :
+  SSA.SSA.atom SSAVM.t -> SSA.SSA.instr -> SSA.SSA.atom SSAVM.t
+
+val subst_map_program_rec :
+  SSA.SSA.atom SSAVM.t -> SSA.SSA.program -> SSA.SSA.atom SSAVM.t
+
+val subst_map_program : SSA.SSA.program -> SSA.SSA.atom SSAVM.t
+
+val subst_map_spec : SSA.SSA.spec -> SSA.SSA.atom SSAVM.t
 
 val rewrite_mov : SSA.SSA.spec -> SSA.SSA.spec
 
