src/SSA2SSALite.v
@@ -29,96 +29,2659 @@ Section VarSubst.
     | Aconst ty n => rconst (sizeof_typ ty) n
     end.
 
-  Fixpoint subst_eexp p r e :=
+  Fixpoint subst_eexp (m : SSAVM.t atom) (e : eexp) : eexp :=
     match e with
-    | Evar v => if v == p then r else e
+    | Evar v => match SSAVM.find v m with
+                | None => e
+                | Some a => eexp_of_atom a
+                end
     | Econst _ => e
-    | Eunop op e => eunary op (subst_eexp p r e)
-    | Ebinop op e1 e2 => ebinary op (subst_eexp p r e1) (subst_eexp p r e2)
-    | Epow e n => epow (subst_eexp p r e) n
+    | Eunop op e => eunary op (subst_eexp m e)
+    | Ebinop op e1 e2 => ebinary op (subst_eexp m e1) (subst_eexp m e2)
+    | Epow e n => epow (subst_eexp m e) n
     end.
 
-  Fixpoint subst_rexp p r e :=
+  Fixpoint subst_rexp (m : SSAVM.t atom) (e : rexp) : rexp :=
     match e with
-    | Rvar v => if v == p then r else e
+    | Rvar v => match SSAVM.find v m with
+                | None => e
+                | Some a => rexp_of_atom a
+                end
     | Rconst _ _ => e
-    | Runop w op e => runary w op (subst_rexp p r e)
-    | Rbinop w op e1 e2 => rbinary w op (subst_rexp p r e1) (subst_rexp p r e2)
-    | Ruext w e i => ruext w (subst_rexp p r e) i
-    | Rsext w e i => rsext w (subst_rexp p r e) i
+    | Runop w op e => runary w op (subst_rexp m e)
+    | Rbinop w op e1 e2 => rbinary w op (subst_rexp m e1) (subst_rexp m e2)
+    | Ruext w e i => ruext w (subst_rexp m e) i
+    | Rsext w e i => rsext w (subst_rexp m e) i
     end.
 
-  Fixpoint subst_eexps p r es :=
-    match es with
-    | [::] => [::]
-    | e::es => (subst_eexp p r e)::(subst_eexps p r es)
-    end.
+  Definition subst_eexps (m : SSAVM.t atom) (es : seq eexp) : seq eexp :=
+    tmap (subst_eexp m) es.
 
-  Fixpoint subst_ebexp p r e :=
+  Fixpoint subst_ebexp (m : SSAVM.t atom) (e : ebexp) : ebexp :=
     match e with
     | Etrue => e
-    | Eeq e1 e2 => Eeq (subst_eexp p r e1) (subst_eexp p r e2)
-    | Eeqmod e1 e2 ms => Eeqmod (subst_eexp p r e1) (subst_eexp p r e2) (subst_eexps p r ms)
-    | Eand e1 e2 => Eand (subst_ebexp p r e1) (subst_ebexp p r e2)
+    | Eeq e1 e2 => Eeq (subst_eexp m e1) (subst_eexp m e2)
+    | Eeqmod e1 e2 ms => Eeqmod (subst_eexp m e1) (subst_eexp m e2) (subst_eexps m ms)
+    | Eand e1 e2 => Eand (subst_ebexp m e1) (subst_ebexp m e2)
     end.
 
-  Fixpoint subst_rbexp p r e :=
+  Fixpoint subst_rbexp (m : SSAVM.t atom) (e : rbexp) : rbexp :=
     match e with
     | Rtrue => e
-    | Req w e1 e2 => Req w (subst_rexp p r e1) (subst_rexp p r e2)
-    | Rcmp w op e1 e2 => Rcmp w op (subst_rexp p r e1) (subst_rexp p r e2)
-    | Rneg e => Rneg (subst_rbexp p r e)
-    | Rand e1 e2 => Rand (subst_rbexp p r e1) (subst_rbexp p r e2)
-    | Ror e1 e2 => Ror (subst_rbexp p r e1) (subst_rbexp p r e2)
+    | Req w e1 e2 => Req w (subst_rexp m e1) (subst_rexp m e2)
+    | Rcmp w op e1 e2 => Rcmp w op (subst_rexp m e1) (subst_rexp m e2)
+    | Rneg e => Rneg (subst_rbexp m e)
+    | Rand e1 e2 => Rand (subst_rbexp m e1) (subst_rbexp m e2)
+    | Ror e1 e2 => Ror (subst_rbexp m e1) (subst_rbexp m e2)
     end.
 
-  Definition subst_bexp p r e :=
-    (subst_ebexp p (eexp_of_atom r) (fst e), subst_rbexp p (rexp_of_atom r) (snd e)).
+  Definition subst_bexp (m : SSAVM.t atom) (e : bexp) : bexp :=
+    (subst_ebexp m (fst e), subst_rbexp m (snd e)).
 
-  Definition subst_atom p r (a : SSA.atom) :=
+  Definition subst_atom (m : SSAVM.t atom) (a : atom) : atom :=
     match a with
-    | Avar v => if v == p then r else a
+    | Avar v => match SSAVM.find v m with
+                | None => a
+                | Some a' => a'
+                end
     | Aconst _ _ => a
     end.
 
-  Definition subst_instr p r i :=
+  Definition subst_instr (m : SSAVM.t atom) (i : instr) : instr :=
     match i with
-    | Imov v a => Imov v (subst_atom p r a)
-    | Ishl v a n => Ishl v (subst_atom p r a) n
-    | Icshl v1 v2 a1 a2 n => Icshl v1 v2 (subst_atom p r a1) (subst_atom p r a2) n
+    | Imov v a => Imov v (subst_atom m a)
+    | Ishl v a n => Ishl v (subst_atom m a) n
+    | Icshl v1 v2 a1 a2 n => Icshl v1 v2 (subst_atom m a1) (subst_atom m a2) n
     | Inondet v t => i
-    | Icmov v c a1 a2 => Icmov v c (subst_atom p r a1) (subst_atom p r a2)
+    | Icmov v c a1 a2 => Icmov v c (subst_atom m a1) (subst_atom m a2)
     | Inop => i
-    | Inot v t a => Inot v t (subst_atom p r a)
-    | Iadd v a1 a2 => Iadd v (subst_atom p r a1) (subst_atom p r a2)
-    | Iadds c v a1 a2 => Iadds c v (subst_atom p r a1) (subst_atom p r a2)
-    | Iadc v a1 a2 y => Iadc v (subst_atom p r a1) (subst_atom p r a2) y
-    | Iadcs c v a1 a2 y => Iadcs c v (subst_atom p r a1) (subst_atom p r a2) y
-    | Isub v a1 a2 => Isub v (subst_atom p r a1) (subst_atom p r a2)
-    | Isubc c v a1 a2 => Isubc c v (subst_atom p r a1) (subst_atom p r a2)
-    | Isubb c v a1 a2 => Isubb c v (subst_atom p r a1) (subst_atom p r a2)
-    | Isbc v a1 a2 y => Isbc v (subst_atom p r a1) (subst_atom p r a2) y
-    | Isbcs c v a1 a2 y => Isbcs c v (subst_atom p r a1) (subst_atom p r a2) y
-    | Isbb v a1 a2 y => Isbb v (subst_atom p r a1) (subst_atom p r a2) y
-    | Isbbs c v a1 a2 y => Isbbs c v (subst_atom p r a1) (subst_atom p r a2) y
-    | Imul v a1 a2 => Imul v (subst_atom p r a1) (subst_atom p r a2)
-    | Imull vh vl a1 a2 => Imull vh vl (subst_atom p r a1) (subst_atom p r a2)
-    | Imulj v a1 a2 => Imulj v (subst_atom p r a1) (subst_atom p r a2)
-    | Isplit vh vl a n => Isplit vh vl (subst_atom p r a) n
-    | Iand v t a1 a2 => Iand v t (subst_atom p r a1) (subst_atom p r a2)
-    | Ior v t a1 a2 => Ior v t (subst_atom p r a1) (subst_atom p r a2)
-    | Ixor v t a1 a2 => Ixor v t (subst_atom p r a1) (subst_atom p r a2)
-    | Icast v t a => Icast v t (subst_atom p r a)
-    | Ivpc v t a => Ivpc v t (subst_atom p r a)
-    | Ijoin v ah al => Ijoin v (subst_atom p r ah) (subst_atom p r al)
-    | Icut e => Icut (subst_bexp p r e)
-    | Iassert e => Iassert (subst_bexp p r e)
-    | Iassume e => Iassume (subst_bexp p r e)
+    | Inot v t a => Inot v t (subst_atom m a)
+    | Iadd v a1 a2 => Iadd v (subst_atom m a1) (subst_atom m a2)
+    | Iadds c v a1 a2 => Iadds c v (subst_atom m a1) (subst_atom m a2)
+    | Iadc v a1 a2 y => Iadc v (subst_atom m a1) (subst_atom m a2) y
+    | Iadcs c v a1 a2 y => Iadcs c v (subst_atom m a1) (subst_atom m a2) y
+    | Isub v a1 a2 => Isub v (subst_atom m a1) (subst_atom m a2)
+    | Isubc c v a1 a2 => Isubc c v (subst_atom m a1) (subst_atom m a2)
+    | Isubb c v a1 a2 => Isubb c v (subst_atom m a1) (subst_atom m a2)
+    | Isbc v a1 a2 y => Isbc v (subst_atom m a1) (subst_atom m a2) y
+    | Isbcs c v a1 a2 y => Isbcs c v (subst_atom m a1) (subst_atom m a2) y
+    | Isbb v a1 a2 y => Isbb v (subst_atom m a1) (subst_atom m a2) y
+    | Isbbs c v a1 a2 y => Isbbs c v (subst_atom m a1) (subst_atom m a2) y
+    | Imul v a1 a2 => Imul v (subst_atom m a1) (subst_atom m a2)
+    | Imull vh vl a1 a2 => Imull vh vl (subst_atom m a1) (subst_atom m a2)
+    | Imulj v a1 a2 => Imulj v (subst_atom m a1) (subst_atom m a2)
+    | Isplit vh vl a n => Isplit vh vl (subst_atom m a) n
+    | Iand v t a1 a2 => Iand v t (subst_atom m a1) (subst_atom m a2)
+    | Ior v t a1 a2 => Ior v t (subst_atom m a1) (subst_atom m a2)
+    | Ixor v t a1 a2 => Ixor v t (subst_atom m a1) (subst_atom m a2)
+    | Icast v t a => Icast v t (subst_atom m a)
+    | Ivpc v t a => Ivpc v t (subst_atom m a)
+    | Ijoin v ah al => Ijoin v (subst_atom m ah) (subst_atom m al)
+    | Icut e => Icut (subst_bexp m e)
+    | Iassert e => Iassert (subst_bexp m e)
+    | Iassume e => Iassume (subst_bexp m e)
     end.
 
-  Definition subst_program p r prog := tmap (subst_instr p r) prog.
+  Definition subst_program (m : SSAVM.t atom) (p : program) : program :=
+    tmap (subst_instr m) p.
+
+  Definition subst_spec (m : SSAVM.t atom) (s : spec) : spec :=
+    {| sinputs := sinputs s;
+       spre := subst_bexp m (spre s);
+       sprog := subst_program m (sprog s);
+       spost := subst_bexp m (spost s) |}.
+
+
+  Lemma vars_eexp_of_atom a : vars_eexp (eexp_of_atom a) = vars_atom a.
+  Proof. by case: a => [ v | ty bs ] //=. Qed.
+
+  Lemma vars_rexp_of_atom a : vars_rexp (rexp_of_atom a) = vars_atom a.
+  Proof. by case: a => [ v | ty bs ] //=. Qed.
+
+  Lemma subst_eexps_cons m e es :
+    subst_eexps m (e::es) = (subst_eexp m e)::(subst_eexps m es).
+  Proof. rewrite /subst_eexps !tmap_map /=. reflexivity. Qed.
+
+  Lemma subst_eexps_rcons m es e :
+    subst_eexps m (rcons es e) = rcons (subst_eexps m es) (subst_eexp m e).
+  Proof. rewrite /subst_eexps !tmap_map. rewrite map_rcons. reflexivity. Qed.
+
+  Lemma subst_eexps_cat m es1 es2 :
+    subst_eexps m (es1 ++ es2) = subst_eexps m es1 ++ subst_eexps m es2.
+  Proof.
+    elim: es1 => [| e1 es1 IH1] //=. rewrite !subst_eexps_cons IH1.
+    rewrite cat_cons. reflexivity.
+  Qed.
+
+  Lemma subst_program_cons m i p :
+    subst_program m (i::p) = (subst_instr m i)::(subst_program m p).
+  Proof. rewrite /subst_program !tmap_map /=. reflexivity. Qed.
+
+  Lemma subst_program_rcons m p i :
+    subst_program m (rcons p i) = rcons (subst_program m p) (subst_instr m i).
+  Proof. rewrite /subst_program !tmap_map. rewrite map_rcons. reflexivity. Qed.
+
+  Lemma subst_program_cat m p1 p2 :
+    subst_program m (p1 ++ p2) = subst_program m p1 ++ subst_program m p2.
+  Proof.
+    elim: p1 => [| i1 p1 IH1] //=. rewrite !subst_program_cons IH1.
+    rewrite cat_cons. reflexivity.
+  Qed.
+
+
+  (* Unchanged substitution *)
+
+  Lemma disjoint_subst_eexp m e :
+    SSAVS.Lemmas.disjoint (TEKS.key_set m) (vars_eexp e) ->
+    subst_eexp m e = e.
+  Proof.
+    elim: e => //=.
+    - move=> v Hdisj. rewrite SSAVS.Lemmas.disjoint_singleton_r in Hdisj.
+      rewrite (TEKS.not_mem_key_set_find Hdisj). reflexivity.
+    - move=> op e IH Hdisj. rewrite (IH Hdisj). reflexivity.
+    - move=> op e1 IH1 e2 IH2 Hdisj. rewrite SSAVS.Lemmas.disjoint_union_r in Hdisj.
+      move/andP: Hdisj => [Hdisj1 Hdisj2]. rewrite (IH1 Hdisj1) (IH2 Hdisj2).
+      reflexivity.
+    - move=> e IH n Hdisj. rewrite (IH Hdisj). reflexivity.
+  Qed.
+
+  Lemma disjoint_subst_rexp m e :
+    SSAVS.Lemmas.disjoint (TEKS.key_set m) (vars_rexp e) ->
+    subst_rexp m e = e.
+  Proof.
+    elim: e => //=.
+    - move=> v Hdisj. rewrite SSAVS.Lemmas.disjoint_singleton_r in Hdisj.
+      rewrite (TEKS.not_mem_key_set_find Hdisj). reflexivity.
+    - move=> w op e IH Hdisj. rewrite (IH Hdisj). reflexivity.
+    - move=> w op e1 IH1 e2 IH2 Hdisj. rewrite SSAVS.Lemmas.disjoint_union_r in Hdisj.
+      move/andP: Hdisj => [Hdisj1 Hdisj2]. rewrite (IH1 Hdisj1) (IH2 Hdisj2).
+      reflexivity.
+    - move=> w e IH n Hdisj. rewrite (IH Hdisj). reflexivity.
+    - move=> w e IH n Hdisj. rewrite (IH Hdisj). reflexivity.
+  Qed.
+
+  Lemma disjoint_subst_eexps m es :
+    SSAVS.Lemmas.disjoint (TEKS.key_set m) (vars_eexps es) ->
+    subst_eexps m es = es.
+  Proof.
+    elim: es => [| e es IH] //=. move=> Hdisj.
+    rewrite SSAVS.Lemmas.disjoint_union_r in Hdisj. move/andP: Hdisj => [Hdisj1 Hdisj2].
+    rewrite subst_eexps_cons. rewrite (disjoint_subst_eexp Hdisj1) (IH Hdisj2).
+    reflexivity.
+  Qed.
+
+  Lemma disjoint_subst_ebexp m e :
+    SSAVS.Lemmas.disjoint (TEKS.key_set m) (vars_ebexp e) ->
+    subst_ebexp m e = e.
+  Proof.
+    elim: e => //=.
+    - move=> e1 e2 Hdisj. rewrite SSAVS.Lemmas.disjoint_union_r in Hdisj.
+      move/andP: Hdisj => [Hdisj1 Hdisj2].
+      rewrite (disjoint_subst_eexp Hdisj1) (disjoint_subst_eexp Hdisj2).
+      reflexivity.
+    - move=> e1 e2 ms Hdisj. rewrite !SSAVS.Lemmas.disjoint_union_r in Hdisj.
+      move/andP: Hdisj => [Hdisj1 /andP [Hdisj2 Hdisj3]].
+      rewrite (disjoint_subst_eexp Hdisj1) (disjoint_subst_eexp Hdisj2)
+              (disjoint_subst_eexps Hdisj3).
+      reflexivity.
+    - move=> e1 IH1 e2 IH2 Hdisj. rewrite SSAVS.Lemmas.disjoint_union_r in Hdisj.
+      move/andP: Hdisj => [Hdisj1 Hdisj2]. rewrite (IH1 Hdisj1) (IH2 Hdisj2).
+      reflexivity.
+  Qed.
+
+  Lemma disjoint_subst_rbexp m e :
+    SSAVS.Lemmas.disjoint (TEKS.key_set m) (vars_rbexp e) ->
+    subst_rbexp m e = e.
+  Proof.
+    elim: e => //=.
+    - move=> w e1 e2 Hdisj. rewrite SSAVS.Lemmas.disjoint_union_r in Hdisj.
+      move/andP: Hdisj => [Hdisj1 Hdisj2].
+      rewrite (disjoint_subst_rexp Hdisj1) (disjoint_subst_rexp Hdisj2).
+      reflexivity.
+    - move=> w op e1 e2 Hdisj. rewrite !SSAVS.Lemmas.disjoint_union_r in Hdisj.
+      move/andP: Hdisj => [Hdisj1 Hdisj2].
+      rewrite (disjoint_subst_rexp Hdisj1) (disjoint_subst_rexp Hdisj2).
+      reflexivity.
+    - move=> e IH Hdisj. rewrite (IH Hdisj). reflexivity.
+    - move=> e1 IH1 e2 IH2 Hdisj. rewrite !SSAVS.Lemmas.disjoint_union_r in Hdisj.
+      move/andP: Hdisj => [Hdisj1 Hdisj2]. rewrite (IH1 Hdisj1) (IH2 Hdisj2).
+      reflexivity.
+    - move=> e1 IH1 e2 IH2 Hdisj. rewrite !SSAVS.Lemmas.disjoint_union_r in Hdisj.
+      move/andP: Hdisj => [Hdisj1 Hdisj2]. rewrite (IH1 Hdisj1) (IH2 Hdisj2).
+      reflexivity.
+  Qed.
+
+  Lemma disjoint_subst_bexp m e :
+    SSAVS.Lemmas.disjoint (TEKS.key_set m) (vars_bexp e) ->
+    subst_bexp m e = e.
+  Proof.
+    case: e => [e r]. rewrite /vars_bexp /subst_bexp /=.
+    rewrite SSAVS.Lemmas.disjoint_union_r => /andP [Hdisj1 Hdisj2].
+    rewrite (disjoint_subst_ebexp Hdisj1) (disjoint_subst_rbexp Hdisj2).
+    reflexivity.
+  Qed.
+
+  Lemma disjoint_subst_atom m a :
+    SSAVS.Lemmas.disjoint (TEKS.key_set m) (vars_atom a) ->
+    subst_atom m a = a.
+  Proof.
+    case: a => //=. move=> v Hdisj. rewrite SSAVS.Lemmas.disjoint_singleton_r in Hdisj.
+    rewrite (TEKS.not_mem_key_set_find Hdisj). reflexivity.
+  Qed.
+
+  Lemma disjoint_subst_instr m i :
+    SSAVS.Lemmas.disjoint (TEKS.key_set m) (rvs_instr i) ->
+    subst_instr m i = i.
+  Proof.
+    (case: i => //=); intros;
+    repeat
+      match goal with
+      | H : is_true (SSAVS.Lemmas.disjoint _ (SSAVS.union _ _)) |- _ =>
+          let H1 := fresh in
+          let H2 := fresh in
+          rewrite SSAVS.Lemmas.disjoint_union_r in H;
+          move/andP: H => [H1 H2]
+      | H : is_true (SSAVS.Lemmas.disjoint _ (vars_atom ?a)) |- context [subst_atom _ ?a] =>
+          rewrite (disjoint_subst_atom H)
+      | H : is_true (SSAVS.Lemmas.disjoint _ (vars_bexp ?e)) |- context [subst_bexp _ ?e] =>
+          rewrite (disjoint_subst_bexp H)
+      end; reflexivity.
+  Qed.
+
+  Lemma disjoint_subst_program m p :
+    SSAVS.Lemmas.disjoint (TEKS.key_set m) (rvs_program p) ->
+    subst_program m p = p.
+  Proof.
+    elim: p => [| i p IH] //=. rewrite SSAVS.Lemmas.disjoint_union_r.
+    move/andP=> [Hdisj1 Hdisj2]. rewrite subst_program_cons.
+    rewrite (disjoint_subst_instr Hdisj1) (IH Hdisj2). reflexivity.
+  Qed.
+
+
+  (* Unchanged evaluation *)
+
+  Definition consistent_value (m : SSAVM.t atom) (s : SSAStore.t) : Prop :=
+    forall x a, SSAVM.find x m = Some a -> SSAStore.acc x s = eval_atom a s.
+
+  Definition consistent_type (m : SSAVM.t atom) (E : SSATE.env) : Prop :=
+    forall x a, SSAVM.find x m = Some a ->
+                is_defined x E
+                /\ are_defined (vars_atom a) E
+                /\ well_typed_atom E a
+                /\ SSATE.vtyp x E = atyp a E.
+
+
+  Lemma consistent_value_empty s : consistent_value (SSAVM.empty _) s.
+  Proof.
+    move=> x a Hx. rewrite SSAVM.Lemmas.empty_o in Hx. discriminate.
+  Qed.
+
+  Lemma consistent_value_upd E m s1 s2 v a :
+    consistent_value m s1 ->
+    consistent_type m E ->
+    SSAStore.Upd v a s1 s2 ->
+    ~~ SSAVS.mem v (vars_env E) ->
+    consistent_value m s2.
+  Proof.
+    move=> Hco Hty Hupd Hnotin x ax Hx. move: (Hty _ _ Hx) => [Hdv [Hdav _]].
+    case Hxv: (x == v).
+    - move/eqP: Hxv => ?; subst. move/memdefP: Hdv => Hdv. move/memenvP: Hdv => Hdv.
+      rewrite Hdv in Hnotin. discriminate.
+    - move/idP/negP: Hxv => Hxv. rewrite (SSAStore.acc_Upd_neq Hxv Hupd).
+      rewrite (Hco _ _ Hx). symmetry. apply: (Upd_disjoint_eval_atom Hupd).
+      move/defsubP: Hdav => Hsub. move: (VSLemmas.not_mem_subset Hnotin Hsub).
+      rewrite VSLemmas.disjoint_singleton_l. by apply.
+  Qed.
+
+  Lemma consistent_value_upd2 E m s1 s2 v1 a1 v2 a2 :
+    consistent_value m s1 ->
+    consistent_type m E ->
+    SSAStore.Upd2 v1 a1 v2 a2 s1 s2 ->
+    ~~ SSAVS.mem v1 (vars_env E) ->
+    ~~ SSAVS.mem v2 (vars_env E) ->
+    consistent_value m s2.
+  Proof.
+    move=> Hco Hty Hupd Hnotin1 Hnotin2 x ax Hx. move: (Hty _ _ Hx) => [Hdv [Hdav _]].
+    case Hxv2: (x == v2).
+    - move/eqP: Hxv2 => ?; subst. move/memdefP: Hdv => Hdv. move/memenvP: Hdv => Hdv.
+      rewrite Hdv in Hnotin2. discriminate.
+    - move/idP/negP: Hxv2 => Hxv2. case Hxv1: (x == v1).
+      + move/eqP: Hxv1 => ?; subst. move/memdefP: Hdv => Hdv. move/memenvP: Hdv => Hdv.
+        rewrite Hdv in Hnotin1. discriminate.
+      + move/idP/negP: Hxv1 => Hxv1. rewrite (SSAStore.acc_Upd2_neq Hxv1 Hxv2 Hupd).
+        rewrite (Hco _ _ Hx). move/defsubP: Hdav => Hsub. symmetry.
+        apply: (Upd2_disjoint_eval_atom Hupd).
+        * rewrite VSLemmas.disjoint_singleton_l.
+          exact: (VSLemmas.not_mem_subset Hnotin1 Hsub).
+        * rewrite VSLemmas.disjoint_singleton_l.
+          exact: (VSLemmas.not_mem_subset Hnotin2 Hsub).
+  Qed.
+
+  Lemma consistent_add m v a s :
+    SSAStore.acc v s = eval_atom a s ->
+    consistent_value m s ->
+    consistent_value (SSAVM.add v a m) s.
+  Proof.
+    move=> Hacc Hco x ax Hx. case Hxv: (x == v).
+    - move/eqP: Hxv => ?; subst. rewrite (SSAVM.Lemmas.find_add_eq (eqxx _)) in Hx.
+      case: Hx => ?; subst. assumption.
+    - move/negP: Hxv => Hxv. rewrite (SSAVM.Lemmas.find_add_neq Hxv) in Hx.
+      rewrite (Hco _ _ Hx). reflexivity.
+  Qed.
+
+  Lemma consistent_value_add_upd E m v a bs s1 s2 :
+    eval_atom a s2 = bs ->
+    SSAStore.Upd v bs s1 s2 ->
+    consistent_type m E ->
+    ~~ SSAVS.mem v (vars_env E) ->
+    consistent_value m s1 ->
+    consistent_value (SSAVM.add v a m) s2.
+  Proof.
+    move=> Heva Hupd Hty Hnotin Hco x ax Hx. case Hxv: (x == v).
+    - move/eqP: Hxv => ?; subst. rewrite (SSAVM.Lemmas.find_add_eq (eqxx _)) in Hx.
+      case: Hx => ?; subst. rewrite (SSAStore.acc_Upd_eq (eqxx _) Hupd). reflexivity.
+    - move/negP: Hxv => Hxv. rewrite (SSAVM.Lemmas.find_add_neq Hxv) in Hx.
+      move/negP: Hxv => Hxv. rewrite (SSAStore.acc_Upd_neq Hxv Hupd).
+      rewrite (Hco _ _ Hx). symmetry. apply: (Upd_disjoint_eval_atom Hupd).
+      rewrite VSLemmas.disjoint_singleton_l. apply/negP=> Hmem.
+      apply/idP: Hnotin. apply: (VSLemmas.mem_subset Hmem).
+      apply/defsubP. exact: (proj1 (proj2 (Hty _ _ Hx))).
+  Qed.
+
+  Lemma consistent_type_empty E : consistent_type (SSAVM.empty _) E.
+  Proof.
+    move=> x a Hx. rewrite SSAVM.Lemmas.empty_o in Hx. discriminate.
+  Qed.
+
+  Lemma consistent_type_subst_atom E m a :
+    consistent_type m E ->
+    atyp (subst_atom m a) E = atyp a E.
+  Proof.
+    move=> Hco. case: a => //=. move=> v. case Hv: (SSAVM.find v m) => //=.
+    move: (proj2 (proj2 (proj2 (Hco _ _ Hv)))). symmetry. assumption.
+  Qed.
+
+  Lemma eval_eexp_of_atom E a s :
+    eval_eexp (eexp_of_atom a) E s = bv2z (atyp a E) (eval_atom a s).
+  Proof. by case: a => //=. Qed.
+
+  Lemma eval_rexp_of_atom a s :
+    eval_rexp (rexp_of_atom a) s = eval_atom a s.
+  Proof. by case: a => //=. Qed.
+
+  Lemma subst_eexp_eval_unchanged E m e s :
+    consistent_value m s ->
+    consistent_type m E ->
+    eval_eexp (subst_eexp m e) E s = eval_eexp e E s.
+  Proof.
+    move=> Hev Hty. elim: e => //=.
+    - move=> v. case Hv: (SSAVM.find v m).
+      + rewrite eval_eexp_of_atom. rewrite /acc2z.
+        rewrite (Hev _ _ Hv) (proj2 (proj2 (proj2 (Hty _ _ Hv)))). reflexivity.
+      + reflexivity.
+    - move=> op e IH. rewrite IH. reflexivity.
+    - move=> op e1 IH1 e2 IH2. rewrite IH1 IH2. reflexivity.
+    - move=> e IH n. rewrite IH. reflexivity.
+  Qed.
+
+  Lemma subst_rexp_eval_unchanged m e s :
+    consistent_value m s ->
+    eval_rexp (subst_rexp m e) s = eval_rexp e s.
+  Proof.
+    move=> Hev. elim: e => //=.
+    - move=> v. case Hv: (SSAVM.find v m).
+      + rewrite eval_rexp_of_atom. rewrite /acc2z.
+        rewrite (Hev _ _ Hv). reflexivity.
+      + reflexivity.
+    - move=> _ op e IH. rewrite IH. reflexivity.
+    - move=> _ op e1 IH1 e2 IH2. rewrite IH1 IH2. reflexivity.
+    - move=> _ e IH n. rewrite IH. reflexivity.
+    - move=> _ e IH n. rewrite IH. reflexivity.
+  Qed.
+
+  Lemma subst_eexps_eval_unchanged E m es s :
+    consistent_value m s ->
+    consistent_type m E ->
+    eval_eexps (subst_eexps m es) E s = eval_eexps es E s.
+  Proof.
+    move=> Hev Hty. elim: es => [| e es IH] //=. rewrite subst_eexps_cons /=.
+    rewrite (subst_eexp_eval_unchanged _ Hev Hty) IH. reflexivity.
+  Qed.
+
+  Lemma subst_ebexp_eval_unchanged E m e s :
+    consistent_value m s ->
+    consistent_type m E ->
+    eval_ebexp (subst_ebexp m e) E s <-> eval_ebexp e E s.
+  Proof.
+    move=> Hev Hty. elim: e => //=.
+    - move=> e1 e2. rewrite !(subst_eexp_eval_unchanged _ Hev Hty). tauto.
+    - move=> e1 e2 ms. rewrite !(subst_eexp_eval_unchanged _ Hev Hty)
+                               (subst_eexps_eval_unchanged _ Hev Hty). tauto.
+    - move=> e1 IH1 e2 IH2. tauto.
+  Qed.
+
+  Lemma subst_rbexp_eval_unchanged m e s :
+    consistent_value m s ->
+    eval_rbexp (subst_rbexp m e) s = eval_rbexp e s.
+  Proof.
+    move=> Hev. elim: e => //=.
+    - move=> _ e1 e2. rewrite !(subst_rexp_eval_unchanged _ Hev). reflexivity.
+    - move=> _ op e1 e2. rewrite !(subst_rexp_eval_unchanged _ Hev). reflexivity.
+    - move=> e IH. rewrite IH. reflexivity.
+    - move=> e1 IH1 e2 IH2. rewrite IH1 IH2. reflexivity.
+    - move=> e1 IH1 e2 IH2. rewrite IH1 IH2. reflexivity.
+  Qed.
+
+  Lemma subst_bexp_eval_unchanged E m e s :
+    consistent_value m s ->
+    consistent_type m E ->
+    eval_bexp (subst_bexp m e) E s <-> eval_bexp e E s.
+  Proof.
+    move=> Hev Hty. case: e => [e r] /=. rewrite /subst_bexp /eval_bexp /=.
+    rewrite (subst_ebexp_eval_unchanged _ Hev Hty) (subst_rbexp_eval_unchanged _ Hev).
+    tauto.
+  Qed.
+
+  Global Instance add_proper_consistent_value_map :
+    Proper (SSAVM.Equal ==> eq ==> iff) consistent_value.
+  Proof.
+    move=> m1 m2 Heq s1 s2 ?; subst. split => Hco x a Hx.
+    - rewrite -Heq in Hx. exact: (Hco _ _ Hx).
+    - rewrite Heq in Hx. exact: (Hco _ _ Hx).
+  Qed.
+
+  Global Instance add_proper_consistent_value_store :
+    Proper (eq ==> SSAStore.Equal ==> iff) consistent_value.
+  Proof.
+    move=> m1 m2 ? s1 s2 Heq; subst. split => Hco x a Hx.
+    - move: (Hco _ _ Hx). rewrite Heq. by apply.
+    - move: (Hco _ _ Hx). rewrite Heq. by apply.
+  Qed.
+
+  Global Instance add_proper_consistent_type_map :
+    Proper (SSAVM.Equal ==> eq ==> iff) consistent_type.
+  Proof.
+    move=> m1 m2 Heq s1 s2 ?; subst. split => Hco x a Hx.
+    - rewrite -Heq in Hx. exact: (Hco _ _ Hx).
+    - rewrite Heq in Hx. exact: (Hco _ _ Hx).
+  Qed.
+
+  Global Instance add_proper_consistent_type_env :
+    Proper (eq ==> SSATE.Equal ==> iff) consistent_type.
+  Proof.
+    move=> m1 m2 ? E1 E2 Heq; subst. split => Hco x a Hx.
+    - move: (Hco _ _ Hx). rewrite Heq. tauto.
+    - move: (Hco _ _ Hx). rewrite Heq. tauto.
+  Qed.
+
+
+  (* Well-formedness *)
+
+  Lemma consistent_type_size_of_subst_rexp E m e :
+    consistent_type m E ->
+    well_formed_rexp E e ->
+    size_of_rexp (subst_rexp m e) E = size_of_rexp e E.
+  Proof.
+    move=> Hco. elim: e => //=. move=> v. rewrite /well_formed_rexp /=.
+    rewrite are_defined_singleton => /andP [Hdv Hsv].
+    dcase (SSAVM.find v m); case.
+    - move=> a. case: a => /=.
+      + move=> u Hv. move: (Hco _ _ Hv) => [_ [_ [_ H]]].
+        rewrite 2!SSATE.vtyp_vsize. rewrite H. reflexivity.
+      + move=> ty bs Hv. move: (Hco _ _ Hv) => [_ [_ [_ H]]].
+        rewrite SSATE.vtyp_vsize H. reflexivity.
+    - move=> Hv. rewrite /size_of_rexp /=. reflexivity.
+  Qed.
+
+  Lemma disjoint_well_formed_eexp E m e :
+    VSLemmas.disjoint (vars_eexp e) (TEKS.key_set m) ->
+    well_formed_eexp E (subst_eexp m e) = well_formed_eexp E e.
+  Proof.
+    elim: e => //=.
+    - move=> v Hdisj. rewrite VSLemmas.disjoint_singleton_l in Hdisj.
+      rewrite (TEKS.not_mem_key_set_find Hdisj). reflexivity.
+    - move=> op e1 IH1 e2 IH2. rewrite VSLemmas.disjoint_union_l.
+      move/andP=> [Hdisj1 Hdisj2]. rewrite /ebinary.
+      rewrite !well_formed_eexp_ebinopb. rewrite (IH1 Hdisj1) (IH2 Hdisj2).
+      reflexivity.
+  Qed.
+
+  Lemma consistent_type_disjoint_well_formed_rexp E m e :
+    consistent_type m E ->
+    VSLemmas.disjoint (vars_rexp e) (TEKS.key_set m) ->
+    well_formed_rexp E (subst_rexp m e) = well_formed_rexp E e.
+  Proof.
+    move=> Hco. elim: e => //=.
+    - move=> v Hdisj. rewrite VSLemmas.disjoint_singleton_l in Hdisj.
+      rewrite (TEKS.not_mem_key_set_find Hdisj). reflexivity.
+    - move=> w op e IH Hdisj. rewrite /runary.
+      rewrite !well_formed_rexp_runopb. rewrite (IH Hdisj).
+      case Hwf: (well_formed_rexp E e) => //=.
+      rewrite (consistent_type_size_of_subst_rexp Hco Hwf). reflexivity.
+    - move=> w op e1 IH1 e2 IH2. rewrite VSLemmas.disjoint_union_l.
+      move/andP=> [Hdisj1 Hdisj2]. rewrite /rbinary.
+      rewrite !well_formed_rexp_rbinopb. rewrite (IH1 Hdisj1) (IH2 Hdisj2).
+      case Hwf1: (well_formed_rexp E e1) => //=.
+      case Hwf2: (well_formed_rexp E e2) => //=.
+      rewrite (consistent_type_size_of_subst_rexp Hco Hwf1)
+              (consistent_type_size_of_subst_rexp Hco Hwf2). reflexivity.
+    - move=> w e IH n Hdisj. rewrite /ruext. rewrite 2!well_formed_rexp_ruextb /=.
+      rewrite (IH Hdisj). case Hwf: (well_formed_rexp E e) => //=.
+      rewrite (consistent_type_size_of_subst_rexp Hco Hwf). reflexivity.
+    - move=> w e IH n Hdisj. rewrite /rsext. rewrite 2!well_formed_rexp_rsextb /=.
+      rewrite (IH Hdisj). case Hwf: (well_formed_rexp E e) => //=.
+      rewrite (consistent_type_size_of_subst_rexp Hco Hwf). reflexivity.
+  Qed.
+
+  Lemma disjoint_well_formed_eexps E m es :
+    VSLemmas.disjoint (vars_eexps es) (TEKS.key_set m) ->
+    well_formed_eexps E (subst_eexps m es) = well_formed_eexps E es.
+  Proof.
+    elim: es => [| e es IH] //=. rewrite VSLemmas.disjoint_union_l.
+    move/andP => [Hdisje Hdisjes]. rewrite subst_eexps_cons /=.
+    rewrite (disjoint_well_formed_eexp _ Hdisje) (IH Hdisjes). reflexivity.
+  Qed.
+
+  Lemma disjoint_well_formed_ebexp E m e :
+    VSLemmas.disjoint (vars_ebexp e) (TEKS.key_set m) ->
+    well_formed_ebexp E (subst_ebexp m e) = well_formed_ebexp E e.
+  Proof.
+    elim: e => //=.
+    - move=> e1 e2. rewrite VSLemmas.disjoint_union_l => /andP [Hdisj1 Hdisj2].
+      rewrite !well_formed_ebexp_eeqb.
+      rewrite (disjoint_well_formed_eexp _ Hdisj1) (disjoint_well_formed_eexp _ Hdisj2).
+      reflexivity.
+    - move=> e1 e2 ms. rewrite 2!VSLemmas.disjoint_union_l => /andP [Hdisj1 /andP [Hdisj2 Hdisjms]].
+      rewrite !well_formed_ebexp_eeqmodb.
+      rewrite (disjoint_well_formed_eexp _ Hdisj1) (disjoint_well_formed_eexp _ Hdisj2)
+              (disjoint_well_formed_eexps _ Hdisjms).
+      reflexivity.
+    - move=> e1 IH1 e2 IH2. rewrite VSLemmas.disjoint_union_l.
+      move/andP=> [Hdisj1 Hdisj2]. rewrite 2!well_formed_ebexp_eandb.
+      rewrite (IH1 Hdisj1) (IH2 Hdisj2). reflexivity.
+  Qed.
+
+  Lemma consistent_type_disjoint_well_formed_rbexp E m e :
+    consistent_type m E ->
+    VSLemmas.disjoint (vars_rbexp e) (TEKS.key_set m) ->
+    well_formed_rbexp E (subst_rbexp m e) = well_formed_rbexp E e.
+  Proof.
+    move=> Hco. elim: e => //=.
+    - move=> w e1 e2. rewrite VSLemmas.disjoint_union_l => /andP [Hdisj1 Hdisj2].
+      rewrite 2!well_formed_rbexp_reqb.
+      rewrite (consistent_type_disjoint_well_formed_rexp Hco Hdisj1)
+              (consistent_type_disjoint_well_formed_rexp Hco Hdisj2).
+      case Hwf1: (well_formed_rexp E e1) => //=. case Hwf2: (well_formed_rexp E e2) => //=.
+      rewrite (consistent_type_size_of_subst_rexp Hco Hwf1)
+              (consistent_type_size_of_subst_rexp Hco Hwf2). reflexivity.
+    - move=> w op e1 e2. rewrite VSLemmas.disjoint_union_l => /andP [Hdisj1 Hdisj2].
+      rewrite 2!well_formed_rbexp_rcmpb.
+      rewrite (consistent_type_disjoint_well_formed_rexp Hco Hdisj1)
+              (consistent_type_disjoint_well_formed_rexp Hco Hdisj2).
+      case Hwf1: (well_formed_rexp E e1) => //=. case Hwf2: (well_formed_rexp E e2) => //=.
+      rewrite (consistent_type_size_of_subst_rexp Hco Hwf1)
+              (consistent_type_size_of_subst_rexp Hco Hwf2). reflexivity.
+    - move=> e1 IH1 e2 IH2. rewrite VSLemmas.disjoint_union_l => /andP [Hdisj1 Hdisj2].
+      rewrite 2!well_formed_rbexp_randb. rewrite (IH1 Hdisj1) (IH2 Hdisj2).
+      reflexivity.
+    - move=> e1 IH1 e2 IH2. rewrite VSLemmas.disjoint_union_l => /andP [Hdisj1 Hdisj2].
+      rewrite 2!well_formed_rbexp_rorb. rewrite (IH1 Hdisj1) (IH2 Hdisj2).
+      reflexivity.
+  Qed.
+
+  Lemma disjoint_well_formed_bexp E m e :
+    consistent_type m E ->
+    VSLemmas.disjoint (vars_bexp e) (TEKS.key_set m) ->
+    well_formed_bexp E (subst_bexp m e) = well_formed_bexp E e.
+  Proof.
+    move=> Hco. case: e => [e r]. rewrite /vars_bexp /=.
+    rewrite VSLemmas.disjoint_union_l => /andP [Hdisje Hdisjr].
+    rewrite /subst_bexp 2!well_formed_bexp_split /=.
+    rewrite (disjoint_well_formed_ebexp _ Hdisje)
+            (consistent_type_disjoint_well_formed_rbexp Hco Hdisjr).
+    reflexivity.
+  Qed.
 
 End VarSubst.
+
+
+(* Rewrite mov statements in AST level - to be implemented for optimization *)
+
+Section RewriteMov.
+
+  Import SSA.
+
+  Definition subst_map_instr (m : SSAVM.t atom) (i : instr) : SSAVM.t atom :=
+    match i with
+    | Imov v a =>
+        (* v <- a *)
+        match a with
+        | Avar u => match SSAVM.find u m with
+                    | None =>
+                        (* v <- u *)
+                        SSAVM.add v a m
+                    | Some ua =>
+                        (* v <- u <- ... <- ua *)
+                        SSAVM.add v ua m
+                    end
+        | Aconst _ _ => SSAVM.add v a m
+        end
+    | _ => m
+    end.
+
+  Fixpoint subst_map_program_rec (m : SSAVM.t atom) (p : program) : SSAVM.t atom :=
+    match p with
+    | [::] => m
+    | i::p => subst_map_program_rec (subst_map_instr m i) p
+    end.
+
+  Definition subst_map_program (p : program) : SSAVM.t atom :=
+    subst_map_program_rec (SSAVM.empty atom) p.
+
+  Definition subst_map_spec (s : spec) : SSAVM.t atom :=
+    subst_map_program (sprog s).
+
+  Definition rewrite_mov (s : spec) : spec :=
+    subst_spec (subst_map_spec s) s.
+
+
+  Lemma subst_map_program_rec_cons m i p :
+    subst_map_program_rec m (i::p) = subst_map_program_rec (subst_map_instr m i) p.
+  Proof. reflexivity. Qed.
+
+  Lemma subst_map_program_rec_rcons m p i :
+    subst_map_program_rec m (rcons p i) = subst_map_instr (subst_map_program_rec m p) i.
+  Proof. by elim: p m i => [| j p IH] m i //=. Qed.
+
+  Lemma subst_map_program_rec_cat m p1 p2 :
+    subst_map_program_rec m (p1 ++ p2) = subst_map_program_rec (subst_map_program_rec m p1) p2.
+  Proof. by elim: p1 m p2 => [| i1 p1 IH1] m p2 //=. Qed.
+
+  Lemma subst_map_instr_unchanged_find x m i :
+    ssa_vars_unchanged_instr (SSAVS.singleton x) i ->
+    SSAVM.find x (subst_map_instr m i) = SSAVM.find x m.
+  Proof.
+    (case i => //=). move=> v a Hun.
+    rewrite ssa_unchanged_instr_disjoint_lvs /= in Hun.
+    rewrite VSLemmas.disjoint_singleton_l in Hun.
+    move: (VSLemmas.not_mem_singleton1 Hun) => {Hun}Hne.
+    case: a => [ u | ty bs ] //=.
+    - case Hu: (SSAVM.find u m).
+      + rewrite (SSAVM.Lemmas.find_add_neq Hne). reflexivity.
+      + rewrite (SSAVM.Lemmas.find_add_neq Hne). reflexivity.
+    - rewrite (SSAVM.Lemmas.find_add_neq Hne). reflexivity.
+  Qed.
+
+  Lemma subst_map_program_rec_unchanged_find x m p :
+    ssa_vars_unchanged_program (SSAVS.singleton x) p ->
+    SSAVM.find x (subst_map_program_rec m p) = SSAVM.find x m.
+  Proof.
+    elim: p m => [| i p IH] m //=. move=> Hun.
+    rewrite (IH _ (ssa_unchanged_program_tl Hun)).
+    exact: (subst_map_instr_unchanged_find _ (ssa_unchanged_program_hd Hun)).
+  Qed.
+
+
+  (* Variables of subst_map_instr and subst_map_program *)
+
+  Lemma subst_map_instr_keys_subset m i :
+    SSAVS.subset (SSA.TEKS.key_set (subst_map_instr m i))
+                 (SSAVS.union (SSA.TEKS.key_set m) (lvs_instr i)).
+  Proof.
+    (case: i => //=); intros;
+    repeat
+      match goal with
+      | |- context [match ?a with | Avar _ => _ | Aconst _ _ => _ end] =>
+          case: a; simpl; intros
+      | |- context [match SSAVM.find ?v ?m with | Some _ => _ | None => _ end] =>
+          case: (SSAVM.find v m); simpl; intros
+      | |- context [TEKS.key_set (SSAVM.add ?v ?a ?m)] =>
+          rewrite TEKS.key_set_add /=
+      end; by SSAVS.Lemmas.dp_subset.
+  Qed.
+
+  Lemma subst_map_program_rec_keys_subset m p :
+    SSAVS.subset (SSA.TEKS.key_set (subst_map_program_rec m p))
+                 (SSAVS.union (SSA.TEKS.key_set m) (lvs_program p)).
+  Proof.
+    elim: p m => [| i p IH] m //=.
+    - by SSAVS.Lemmas.dp_subset.
+    - move: (IH (subst_map_instr m i)) => Hsub1.
+      move: (subst_map_instr_keys_subset m i) => Hsub2.
+      move: (VSLemmas.union_subsets Hsub2 (SSAVS.Lemmas.subset_refl (lvs_program p))) => {}Hsub2.
+      apply: (SSAVS.Lemmas.subset_trans Hsub1).
+      apply: (SSAVS.Lemmas.subset_trans Hsub2).
+      by SSAVS.Lemmas.dp_subset.
+  Qed.
+
+  Lemma subst_map_program_keys_subset p :
+    SSAVS.subset (SSA.TEKS.key_set (subst_map_program p))
+                 (lvs_program p).
+  Proof.
+    apply: (SSAVS.Lemmas.subset_trans (subst_map_program_rec_keys_subset _ _)).
+    rewrite TEKS.key_set_empty. by SSAVS.Lemmas.dp_subset.
+  Qed.
+
+  Lemma subst_map_program_keys_disjoint E p :
+    well_formed_ssa_program E p ->
+    VSLemmas.disjoint (TEKS.key_set (subst_map_program p)) (vars_env E).
+  Proof.
+    move=> Hwf.
+    apply: (VSLemmas.disjoint_subset_l _ (subst_map_program_keys_subset p)).
+    rewrite VSLemmas.disjoint_sym. rewrite -ssa_unchanged_program_disjoint_lvs.
+    exact: (well_formed_ssa_unchanged_env Hwf).
+  Qed.
+
+
+  (* Unchanged substitution *)
+
+  Lemma subst_map_instr_find_unchanged m v i :
+    ssa_vars_unchanged_instr (SSAVS.singleton v) i ->
+    SSAVM.find v (subst_map_instr m i) = SSAVM.find v m.
+  Proof.
+    rewrite /subst_map_instr. (case: i => //=).
+    move=> u a. (case: a => //=).
+    - move=> x Hun. rewrite ssa_unchanged_instr_disjoint_lvs /= in Hun.
+      rewrite VSLemmas.disjoint_singleton in Hun.
+      move: (VSLemmas.not_mem_singleton1 Hun) => {Hun} Hne.
+      case Hx: (SSAVM.find x m).
+      + rewrite SSAVM.Lemmas.find_add_neq; first reflexivity.
+        move=> Heq. apply: Hne. symmetry. assumption.
+      + rewrite SSAVM.Lemmas.find_add_neq; first reflexivity.
+        move=> Heq. apply: Hne. symmetry. assumption.
+    - move=> ty bs Hun. rewrite ssa_unchanged_instr_disjoint_lvs /= in Hun.
+      rewrite VSLemmas.disjoint_singleton in Hun.
+      move: (VSLemmas.not_mem_singleton1 Hun) => {Hun} Hne.
+      rewrite SSAVM.Lemmas.find_add_neq; first reflexivity.
+      move=> Heq. apply: Hne. symmetry. assumption.
+  Qed.
+
+  Lemma subst_eexp_subst_map_instr_unchanged m e i :
+    ssa_vars_unchanged_instr (vars_eexp e) i ->
+    subst_eexp (subst_map_instr m i) e = subst_eexp m e.
+  Proof.
+    elim: e => //=.
+    - move=> v Hun. rewrite (subst_map_instr_find_unchanged _ Hun).
+      reflexivity.
+    - move=> op e IH Hun. rewrite (IH Hun). reflexivity.
+    - move=> op e1 IH1 e2 IH2. rewrite ssa_unchanged_instr_union.
+      move/andP => [Hun1 Hun2]. rewrite (IH1 Hun1) (IH2 Hun2). reflexivity.
+    - move=> e IH n Hun. rewrite (IH Hun). reflexivity.
+  Qed.
+
+  Lemma subst_rexp_subst_map_instr_unchanged m e i :
+    ssa_vars_unchanged_instr (vars_rexp e) i ->
+    subst_rexp (subst_map_instr m i) e = subst_rexp m e.
+  Proof.
+    elim: e => //=.
+    - move=> v Hun. rewrite (subst_map_instr_find_unchanged _ Hun).
+      reflexivity.
+    - move=> w op e IH Hun. rewrite (IH Hun). reflexivity.
+    - move=> w op e1 IH1 e2 IH2. rewrite ssa_unchanged_instr_union.
+      move/andP => [Hun1 Hun2]. rewrite (IH1 Hun1) (IH2 Hun2). reflexivity.
+    - move=> w e IH n Hun. rewrite (IH Hun). reflexivity.
+    - move=> w e IH n Hun. rewrite (IH Hun). reflexivity.
+  Qed.
+
+  Lemma subst_eexps_subst_map_instr_unchanged m es i :
+    ssa_vars_unchanged_instr (vars_eexps es) i ->
+    subst_eexps (subst_map_instr m i) es = subst_eexps m es.
+  Proof.
+    elim: es => [| e es IH] //=. rewrite !subst_eexps_cons.
+    rewrite ssa_unchanged_instr_union. move/andP => [Hun1 Hun2].
+    rewrite (subst_eexp_subst_map_instr_unchanged _ Hun1) (IH Hun2). reflexivity.
+  Qed.
+
+  Lemma subst_ebexp_subst_map_instr_unchanged m e i :
+    ssa_vars_unchanged_instr (vars_ebexp e) i ->
+    subst_ebexp (subst_map_instr m i) e = subst_ebexp m e.
+  Proof.
+    elim: e => //=.
+    - move=> e1 e2. rewrite ssa_unchanged_instr_union.
+      move/andP => [Hun1 Hun2]. rewrite (subst_eexp_subst_map_instr_unchanged _ Hun1)
+                                        (subst_eexp_subst_map_instr_unchanged _ Hun2).
+      reflexivity.
+    - move=> e1 e2 ms. rewrite !ssa_unchanged_instr_union.
+      move/andP => [Hun1 /andP [Hun2 Hun3]].
+      rewrite (subst_eexp_subst_map_instr_unchanged _ Hun1)
+              (subst_eexp_subst_map_instr_unchanged _ Hun2)
+              (subst_eexps_subst_map_instr_unchanged _ Hun3).
+      reflexivity.
+    - move=> e1 IH1 e2 IH2. rewrite ssa_unchanged_instr_union.
+      move/andP => [Hun1 Hun2]. rewrite (IH1 Hun1) (IH2 Hun2). reflexivity.
+  Qed.
+
+  Lemma subst_rbexp_subst_map_instr_unchanged m e i :
+    ssa_vars_unchanged_instr (vars_rbexp e) i ->
+    subst_rbexp (subst_map_instr m i) e = subst_rbexp m e.
+  Proof.
+    elim: e => //=.
+    - move=> w e1 e2. rewrite ssa_unchanged_instr_union.
+      move/andP => [Hun1 Hun2]. rewrite (subst_rexp_subst_map_instr_unchanged _ Hun1)
+                                        (subst_rexp_subst_map_instr_unchanged _ Hun2).
+      reflexivity.
+    - move=> w op e1 e2. rewrite ssa_unchanged_instr_union.
+      move/andP => [Hun1 Hun2]. rewrite (subst_rexp_subst_map_instr_unchanged _ Hun1)
+                                        (subst_rexp_subst_map_instr_unchanged _ Hun2).
+      reflexivity.
+    - move=> e IH Hun. rewrite (IH Hun). reflexivity.
+    - move=> e1 IH1 e2 IH2. rewrite ssa_unchanged_instr_union.
+      move/andP => [Hun1 Hun2]. rewrite (IH1 Hun1) (IH2 Hun2). reflexivity.
+    - move=> e1 IH1 e2 IH2. rewrite ssa_unchanged_instr_union.
+      move/andP => [Hun1 Hun2]. rewrite (IH1 Hun1) (IH2 Hun2). reflexivity.
+  Qed.
+
+  Lemma subst_bexp_subst_map_instr_unchanged m e i :
+    ssa_vars_unchanged_instr (vars_bexp e) i ->
+    subst_bexp (subst_map_instr m i) e = subst_bexp m e.
+  Proof.
+    case: e => [e r]. rewrite /vars_bexp /subst_bexp /=.
+    rewrite ssa_unchanged_instr_union. move/andP => [Hun1 Hun2].
+    rewrite (subst_ebexp_subst_map_instr_unchanged _ Hun1)
+            (subst_rbexp_subst_map_instr_unchanged _ Hun2).
+    reflexivity.
+  Qed.
+
+  Lemma subst_atom_subst_map_instr_unchanged m a i :
+    ssa_vars_unchanged_instr (vars_atom a) i ->
+    subst_atom (subst_map_instr m i) a = subst_atom m a.
+  Proof.
+    case: a => //=. move=> v Hun.
+    rewrite (subst_map_instr_find_unchanged _ Hun). reflexivity.
+  Qed.
+
+  Lemma subst_instr_subst_map_instr_unchanged m i j :
+    ssa_vars_unchanged_instr (rvs_instr i) j ->
+    subst_instr (subst_map_instr m j) i = subst_instr m i.
+  Proof.
+    (case: i => //=); intros;
+      by repeat match goal with
+                | H : is_true (ssa_vars_unchanged_instr (SSAVS.union _ _) _) |- _ =>
+                    let H1 := fresh in
+                    let H2 := fresh in
+                    rewrite ssa_unchanged_instr_union in H;
+                    move/andP: H => [H1 H2]
+                | H : is_true (ssa_vars_unchanged_instr (vars_atom ?a) ?j)
+                  |- context [subst_atom (subst_map_instr ?m ?j) ?a] =>
+                    rewrite (subst_atom_subst_map_instr_unchanged _ H)
+                | H : is_true (ssa_vars_unchanged_instr (vars_bexp ?a) ?j)
+                  |- context [subst_bexp (subst_map_instr ?m ?j) ?a] =>
+                    rewrite (subst_bexp_subst_map_instr_unchanged _ H)
+                | |- ?e = ?e => reflexivity
+                end.
+  Qed.
+
+  Lemma subst_instr_subst_map_program_rec_unchanged m i p :
+    ssa_vars_unchanged_program (rvs_instr i) p ->
+    subst_instr (subst_map_program_rec m p) i = subst_instr m i.
+  Proof.
+    elim: p i m => [| j p IH] i m //=. rewrite ssa_unchanged_program_cons.
+    move/andP => [Hunj Hunp]. rewrite (IH _ _ Hunp).
+    exact: (subst_instr_subst_map_instr_unchanged _ Hunj).
+  Qed.
+
+
+  (* consistent_type after subst_map_instr or subst_map_program *)
+
+  Lemma subst_map_instr_consistent_type E m i :
+    well_formed_instr E i ->
+    ssa_vars_unchanged_instr (vars_env E) i ->
+    consistent_type m E ->
+    consistent_type (subst_map_instr m i) (instr_succ_typenv i E).
+  Proof.
+    (case: i => //=); intros;
+    repeat match goal with
+           | H : is_true (well_formed_instr _ _) |- _ =>
+               rewrite /well_formed_instr /= in H
+           | H : is_true (_ && _) |- _ =>
+               let H1 := fresh in
+               let H2 := fresh in
+               move/andP: H => [H1 H2]
+           | H : is_true (ssa_vars_unchanged_instr _ _) |- _ =>
+               rewrite ssa_unchanged_instr_disjoint_lvs /= in H
+           | H : is_true (VSLemmas.disjoint _ (SSAVS.singleton _)) |- _ =>
+               rewrite VSLemmas.disjoint_singleton_r in H
+           | H : is_true (VSLemmas.disjoint _ (SSAVS.add _ _)) |- _ =>
+               let H1 := fresh in
+               let H2 := fresh in
+               (rewrite VSLemmas.disjoint_add_r /= in H);
+               move/andP: H => [H1 H2]
+           | H1 : consistent_type ?m ?E,
+               H0 : is_true (~~ SSAVS.mem ?t (vars_env ?E)) |-
+               consistent_type ?m (SSATE.add ?t _ ?E) =>
+               (move => x ax Hx); simpl; (move: (H1 _ _ Hx) => [Hdefx [Hdefax [Hsmax Htyx]]]); repeat split;
+               [ by rewrite is_defined_add Hdefx orbT
+               | apply: are_defined_addr; exact: Hdefax
+               | (rewrite well_typed_atom_notin_add; first assumption);
+                 apply: (VSLemmas.not_mem_subset H0);
+                 move/defsubP: Hdefax; by apply
+               | rewrite is_defined_mem_vars_env in Hdefx;
+                 (have Hxt: x != t
+                   by apply/negP => /eqP ?; subst; rewrite Hdefx in H0; discriminate);
+                 rewrite (SSATE.vtyp_add_neq Hxt) Htyx;
+                 rewrite atyp_add_not_mem; first reflexivity;
+                 (apply/negP => Hmemt); (move/negP: H0; apply);
+                 (move/defsubP: Hdefax => Hsub); exact: (VSLemmas.mem_subset Hmemt Hsub) ]
+           | H1 : consistent_type ?m ?E,
+               H : is_true (~~ SSAVS.mem ?t (vars_env ?E)),
+                 H10 : is_true (~~ SSAVS.mem ?t0 (vars_env ?E)) |-
+               consistent_type ?m (SSATE.add ?t _ (SSATE.add ?t0 _ ?E)) =>
+               (move => x ax Hx); simpl; (move: (H1 _ _ Hx) => [Hdefx [Hdefax [Hsmax Htyx]]]); repeat split;
+               [ by rewrite !is_defined_add Hdefx !orbT
+               | repeat apply: are_defined_addr; exact: Hdefax
+               | (rewrite well_typed_atom_notin_add;
+                  last by (apply: (VSLemmas.not_mem_subset H); move/defsubP: Hdefax; apply));
+                 (rewrite well_typed_atom_notin_add;
+                  last by (apply: (VSLemmas.not_mem_subset H10); move/defsubP: Hdefax; apply));
+                 assumption
+               | rewrite is_defined_mem_vars_env in Hdefx;
+                 (have Hxt: x != t
+                   by apply/negP => /eqP ?; subst; rewrite Hdefx in H; discriminate);
+                 (have Hxt0: x != t0
+                   by apply/negP => /eqP ?; subst; rewrite Hdefx in H10; discriminate);
+                 rewrite (SSATE.vtyp_add_neq Hxt) (SSATE.vtyp_add_neq Hxt0) Htyx;
+                 rewrite atyp_add_not_mem; [ rewrite atyp_add_not_mem |]; first reflexivity;
+                 [ (apply/negP => Hmemt); (move/negP: H10; apply);
+                   (move/defsubP: Hdefax => Hsub); exact: (VSLemmas.mem_subset Hmemt Hsub)
+                 | (apply/negP => Hmemt); (move/negP: H; apply);
+                   (move/defsubP: Hdefax => Hsub); exact: (VSLemmas.mem_subset Hmemt Hsub) ] ]
+           end.
+    (* Imov *)
+    move: H0 H1 H2 H3 => Hmemt Hty Hdefa Hwta.
+    case: a Hdefa Hwta => //=.
+    - move=> v Hdefv Hwtv. case Hvm: (SSAVM.find v m).
+      + move=> x ax Hx. move: (Hty _ _ Hvm) => [Hdefv' [Hdefa [Hwta Htyv]]].
+        case Hxt: (x == t).
+        * move/eqP: Hxt => ?; subst.
+          rewrite (SSAVM.Lemmas.find_add_eq (eqxx _)) in Hx. case: Hx => ?; subst.
+          repeat split.
+          -- by rewrite is_defined_add eqxx.
+          -- repeat apply: are_defined_addr. exact: Hdefa.
+          -- rewrite well_typed_atom_notin_add; first assumption.
+             apply: (VSLemmas.not_mem_subset Hmemt). move/defsubP: Hdefa. by apply.
+          -- rewrite (SSATE.vtyp_add_eq (eqxx _)). rewrite atyp_add_not_mem; first exact: Htyv.
+             apply/negP=> Hmem. move/negP: Hmemt; apply. move/defsubP: Hdefa => Hsub.
+             exact: (VSLemmas.mem_subset Hmem Hsub).
+        * move/negP: Hxt => Hxt. rewrite (SSAVM.Lemmas.find_add_neq Hxt) in Hx.
+          move: (Hty _ _ Hx) => [Hdefx [Hdefax [Hwtax Htyx]]]. repeat split.
+          -- by rewrite !is_defined_add Hdefx !orbT.
+          -- repeat apply: are_defined_addr; exact: Hdefax.
+          -- rewrite well_typed_atom_notin_add; first assumption.
+             apply: (VSLemmas.not_mem_subset Hmemt). move/defsubP: Hdefax. by apply.
+          -- move/negP: Hxt => Hxt. rewrite (SSATE.vtyp_add_neq Hxt).
+             rewrite atyp_add_not_mem; first exact: Htyx.
+             apply/negP=> Hmem. move/negP: Hmemt; apply. move/defsubP: Hdefax => Hsub.
+             exact: (VSLemmas.mem_subset Hmem Hsub).
+      + move=> x ax Hx. case Hxt: (x == t).
+        * move/eqP: Hxt => ?; subst; simpl.
+          rewrite (SSAVM.Lemmas.find_add_eq (eqxx _)) in Hx. case: Hx => ?; subst; simpl.
+          repeat split.
+          -- by rewrite is_defined_add eqxx.
+          -- repeat apply: are_defined_addr. exact: Hdefv.
+          -- rewrite well_typed_atom_notin_add; first assumption.
+             apply: (VSLemmas.not_mem_subset Hmemt). move/defsubP: Hdefv. by apply.
+          -- rewrite (SSATE.vtyp_add_eq (eqxx _)). rewrite SSATE.vtyp_add_neq; first reflexivity.
+             apply/negP=> /eqP ?; subst. rewrite are_defined_singleton in Hdefv.
+             move/memdefP: Hdefv => Hmem. rewrite mem_vars_env Hmem in Hmemt. discriminate.
+        * move/negP: Hxt => Hxt. rewrite (SSAVM.Lemmas.find_add_neq Hxt) in Hx.
+          move: (Hty _ _ Hx) => [Hdefx [Hdefax [Hsmax Htyx]]]. repeat split.
+          -- by rewrite !is_defined_add Hdefx !orbT.
+          -- repeat apply: are_defined_addr; exact: Hdefax.
+          -- rewrite well_typed_atom_notin_add; first assumption.
+             apply: (VSLemmas.not_mem_subset Hmemt). move/defsubP: Hdefax. by apply.
+          -- move/negP: Hxt => Hxt. rewrite (SSATE.vtyp_add_neq Hxt).
+             rewrite atyp_add_not_mem; first exact: Htyx.
+             apply/negP=> Hmem. move/negP: Hmemt; apply. move/defsubP: Hdefax => Hsub.
+             exact: (VSLemmas.mem_subset Hmem Hsub).
+    - move=> ty bs _ Hwf. move=> x ax Hx. case Hxt: (x == t).
+      + move/eqP: Hxt => ?; subst.
+        rewrite (SSAVM.Lemmas.find_add_eq (eqxx _)) in Hx. case: Hx => ?; subst.
+        repeat split.
+        * by rewrite is_defined_add eqxx.
+        * exact: Hwf.
+        * rewrite (SSATE.vtyp_add_eq (eqxx _)). reflexivity.
+      + move/negP: Hxt => Hxt. rewrite (SSAVM.Lemmas.find_add_neq Hxt) in Hx.
+        move: (Hty _ _ Hx) => [Hdefx [Hdefax [Hsmax Htyx]]]. repeat split.
+        * by rewrite !is_defined_add Hdefx !orbT.
+        * repeat apply: are_defined_addr; exact: Hdefax.
+        * rewrite well_typed_atom_notin_add; first assumption.
+          apply: (VSLemmas.not_mem_subset Hmemt). move/defsubP: Hdefax. by apply.
+        * move/negP: Hxt => Hxt. rewrite (SSATE.vtyp_add_neq Hxt).
+          rewrite atyp_add_not_mem; first exact: Htyx.
+          apply/negP=> Hmem. move/negP: Hmemt; apply. move/defsubP: Hdefax => Hsub.
+          exact: (VSLemmas.mem_subset Hmem Hsub).
+  Qed.
+
+  Lemma subst_map_program_rec_consistent_type E p m :
+    well_formed_ssa_program E p ->
+    consistent_type m E ->
+    consistent_type (subst_map_program_rec m p) (program_succ_typenv p E).
+  Proof.
+    elim: p E m => [| i p IH] E m //=. move=> Hwf Hty.
+    apply: (IH _ _ (well_formed_ssa_tl Hwf)) => {IH}.
+    exact: (subst_map_instr_consistent_type
+              (well_formed_ssa_hd Hwf)
+              (well_formed_ssa_unchanged_env_hd Hwf) Hty).
+  Qed.
+
+  Lemma subst_map_program_consistent_type E p :
+    well_formed_ssa_program E p ->
+    consistent_type (subst_map_program p) (program_succ_typenv p E).
+  Proof.
+    move=> Hwf. exact: (subst_map_program_rec_consistent_type Hwf (consistent_type_empty _)).
+  Qed.
+
+
+  (* Typing environments after subst_instr or subst_program *)
+
+  Lemma consistent_type_instr_succ_typenv E m i :
+    consistent_type m E ->
+    SSATE.Equal (instr_succ_typenv (subst_instr m i) E)
+                (instr_succ_typenv i E).
+  Proof.
+    move=> Hco.
+    (case: i => //=); intros;
+      by repeat match goal with
+                | |- SSATE.Equal _ _ => move=> x
+                | |- context [SSAVM.find ?x (SSATE.add ?t _ _)] =>
+                    let Hxt := fresh in
+                    dcase (x == t); case; intro Hxt;
+                    [ (move/eqP: Hxt => ?); subst; rewrite !(SSATE.Lemmas.find_add_eq (eqxx _))
+                    | (move/negP: Hxt => Hxt); rewrite !(SSATE.Lemmas.find_add_neq Hxt) ]
+                | Hco : consistent_type ?m ?E
+                  |- context [atyp (subst_atom ?m ?a) ?E] =>
+                    rewrite (consistent_type_subst_atom _ Hco)
+                | |- ?e = ?e => reflexivity
+                end.
+  Qed.
+
+  Lemma subst_map_program_succ_typenv E p :
+    well_formed_ssa_program E p ->
+    SSATE.Equal (program_succ_typenv (subst_program (subst_map_program p) p) E)
+                (program_succ_typenv p E).
+  Proof.
+    move=> Hwf. rewrite /subst_map_program.
+    move: (consistent_type_empty E). move: (SSAVM.empty atom).
+    elim: p E Hwf => [| i p IH] E Hwf m Hty //=. rewrite subst_program_cons /=.
+    have ->: (subst_instr (subst_map_program_rec (subst_map_instr m i) p) i) =
+           (subst_instr m i).
+    { move: (well_formed_ssa_vars_unchanged_hd Hwf) => Hun.
+      move: (ssa_unchanged_program_subset Hun (rvs_instr_subset i)) => {}Hun.
+      rewrite (subst_instr_subst_map_program_rec_unchanged _ Hun).
+      apply: subst_instr_subst_map_instr_unchanged.
+      exact: (well_formed_ssa_lvs_unchanged_hd Hwf). }
+    rewrite (consistent_type_instr_succ_typenv _ Hty). apply: (IH _ (well_formed_ssa_tl Hwf)).
+    exact: (subst_map_instr_consistent_type
+              (well_formed_ssa_hd Hwf)
+              (well_formed_ssa_unchanged_env_hd Hwf) Hty).
+  Qed.
+
+  Lemma rewrite_mov_succ_typenv s :
+    well_formed_ssa_spec s ->
+    SSATE.Equal
+             (program_succ_typenv (sprog (rewrite_mov s)) (sinputs (rewrite_mov s)))
+             (program_succ_typenv (sprog s) (sinputs s)).
+  Proof.
+    move=> Hwf. apply: (subst_map_program_succ_typenv (well_formed_ssa_spec_program Hwf)).
+  Qed.
+
+
+  (* Consistent evaluation after subst_map_instr or subst_map_program *)
+
+  Lemma subst_map_instr_consistent_value E i m s1 s2 :
+    consistent_type m E ->
+    consistent_value m s1 ->
+    eval_instr E i (OK s1) (OK s2) ->
+    well_formed_instr E i ->
+    ssa_vars_unchanged_instr (vars_env E) i ->
+    consistent_value (subst_map_instr m i) s2.
+  Proof.
+    (move=> Hty Hco Hevi). inversion_clear Hevi; simpl; intros;
+      repeat match goal with
+             | H : is_true (ssa_vars_unchanged_instr _ _) |- _ =>
+                 rewrite ssa_unchanged_instr_disjoint_lvs /= in H
+             | H : is_true (VSLemmas.disjoint _ (SSAVS.singleton _)) |- _ =>
+                 rewrite VSLemmas.disjoint_singleton_r in H
+             | H : is_true (VSLemmas.disjoint _ (SSAVS.add _ _)) |- _ =>
+                 let H1 := fresh in
+                 let H2 := fresh in
+                 rewrite VSLemmas.disjoint_add_r in H;
+                 move/andP: H => [H1 H2]
+             | Hty : consistent_type ?m ?E,
+                 Hco : consistent_value ?m ?s1,
+                   Hupd : SSAStore.Upd ?v _ ?s1 ?s2,
+                     Hnotin : is_true (~~ SSAVS.mem ?v (vars_env ?E))
+               |- consistent_value ?m ?s2 =>
+                 apply: (consistent_value_upd Hco Hty Hupd Hnotin)
+             | Hty : consistent_type ?m ?E,
+                 Hco : consistent_value ?m ?s1,
+                   Hupd : SSAStore.Upd2 ?v1 _ ?v2 _ ?s1 ?s2,
+                     Hnotin1 : is_true (~~ SSAVS.mem ?v1 (vars_env ?E)),
+                       Hnotin2 : is_true (~~ SSAVS.mem ?v2 (vars_env ?E))
+               |- consistent_value ?m ?s2 =>
+                 apply: (consistent_value_upd2 Hco Hty Hupd Hnotin1 Hnotin2)
+             |  Hco : consistent_value ?m ?s1,
+                 Heq : SSAStore.Equal ?s1 ?s2
+                |- consistent_value ?m ?s2 =>
+                  rewrite -Heq; exact: Hco
+             end.
+    (* Imov *)
+    case: a H H0 => //=.
+    - move=> u Hupd Hwf. case Hu: (SSAVM.find u m).
+      + apply: (consistent_value_add_upd _ Hupd Hty H1 Hco).
+        rewrite (Hco _ _ Hu). apply: (Upd_disjoint_eval_atom Hupd).
+        rewrite VSLemmas.disjoint_singleton_l. apply/negP => Hmem.
+        apply/idP: H1. apply: (VSLemmas.mem_subset Hmem). apply/defsubP.
+        exact: (proj1 (proj2 (Hty _ _ Hu))).
+      + apply: (consistent_value_add_upd _ Hupd Hty H1 Hco). simpl.
+        apply: (SSAStore.acc_Upd_neq _ Hupd).
+        apply/negP => /eqP Huv; subst. move/andP: Hwf => /= [Hdef _].
+        move/defsubP: Hdef => Hsub. apply/idP: H1. rewrite SSAVS.Lemmas.subset_singleton in Hsub.
+        exact: Hsub.
+    - move=> ty bs Hupd Hwf. apply: (consistent_value_add_upd _ Hupd Hty H1 Hco).
+      reflexivity.
+  Qed.
+
+  Lemma subst_map_instr_consistent_value' E i m s1 s2 :
+    consistent_type m E ->
+    consistent_value m s1 ->
+    eval_instr E (subst_instr m i) (OK s1) (OK s2) ->
+    well_formed_instr E i ->
+    ssa_vars_unchanged_instr (vars_env E) i ->
+    consistent_value (subst_map_instr m i) s2.
+  Proof.
+    (move=> Hty Hco).
+    (case: i => //=); intros;
+    repeat match goal with
+           | H : eval_instr _ _ _ _ |- _ =>
+               inversion_clear H
+           | H : is_true (ssa_vars_unchanged_instr _ _) |- _ =>
+               rewrite ssa_unchanged_instr_disjoint_lvs /= in H
+           | H : is_true (VSLemmas.disjoint _ (SSAVS.singleton _)) |- _ =>
+               rewrite VSLemmas.disjoint_singleton_r in H
+           | H : is_true (VSLemmas.disjoint _ (SSAVS.add _ _)) |- _ =>
+               let H1 := fresh in
+               let H2 := fresh in
+               rewrite VSLemmas.disjoint_add_r in H;
+               move/andP: H => [H1 H2]
+           | Hty : consistent_type ?m ?E,
+               Hco : consistent_value ?m ?s1,
+                 Hupd : SSAStore.Upd ?v _ ?s1 ?s2,
+                   Hnotin : is_true (~~ SSAVS.mem ?v (vars_env ?E))
+             |- consistent_value ?m ?s2 =>
+               apply: (consistent_value_upd Hco Hty Hupd Hnotin)
+           | Hty : consistent_type ?m ?E,
+               Hco : consistent_value ?m ?s1,
+                 Hupd : SSAStore.Upd2 ?v1 _ ?v2 _ ?s1 ?s2,
+                   Hnotin1 : is_true (~~ SSAVS.mem ?v1 (vars_env ?E)),
+                     Hnotin2 : is_true (~~ SSAVS.mem ?v2 (vars_env ?E))
+             |- consistent_value ?m ?s2 =>
+               apply: (consistent_value_upd2 Hco Hty Hupd Hnotin1 Hnotin2)
+           |  Hco : consistent_value ?m ?s1,
+               Heq : SSAStore.Equal ?s1 ?s2
+              |- consistent_value ?m ?s2 =>
+                rewrite -Heq; exact: Hco
+           end.
+    (* Imov *)
+    case: a H0 H2 => //=.
+    - move=> u Hwf. case Hu: (SSAVM.find u m) => Hupd.
+      + apply: (consistent_value_add_upd _ Hupd Hty H1 Hco).
+        apply: (Upd_disjoint_eval_atom Hupd).
+        rewrite VSLemmas.disjoint_singleton_l. apply/negP => Hmem.
+        apply/idP: H1. apply: (VSLemmas.mem_subset Hmem). apply/defsubP.
+        exact: (proj1 (proj2 (Hty _ _ Hu))).
+      + apply: (consistent_value_add_upd _ Hupd Hty H1 Hco). simpl.
+        apply: (SSAStore.acc_Upd_neq _ Hupd).
+        apply/negP => /eqP Huv; subst. move/andP: Hwf => /= [Hdef _].
+        move/defsubP: Hdef => Hsub. apply/idP: H1. rewrite SSAVS.Lemmas.subset_singleton in Hsub.
+        exact: Hsub.
+    - move=> ty bs Hwf Hupd. apply: (consistent_value_add_upd _ Hupd Hty H1 Hco).
+      reflexivity.
+  Qed.
+
+  Lemma subst_map_program_consistent_value E p s1 s2 :
+    well_formed_ssa_program E p ->
+    eval_program E p (OK s1) (OK s2) ->
+    consistent_value (subst_map_program p) s2.
+  Proof.
+    rewrite /subst_map_program. move: (consistent_value_empty s1).
+    move: (consistent_type_empty E).
+    move: (SSAVM.empty atom). elim: p E s1 s2 => [| i p IH] E s1 s2 m Hty Hco Hwf Hev //=.
+    - inversion_clear Hev. move: H => Heq. simpl in Heq. rewrite -Heq. exact: Hco.
+    - inversion_clear Hev. move: H H0 => Hevi Hevp.
+      move: (well_formed_ssa_hd Hwf) => Hwfi.
+      move: (well_formed_ssa_unchanged_env_hd Hwf) => HunEi.
+      case: t Hevi Hevp => [ t |] Hevi Hevp.
+      + apply: (IH _ t _ _
+                   (subst_map_instr_consistent_type Hwfi HunEi Hty)
+                   _ (well_formed_ssa_tl Hwf) Hevp).
+        exact: (subst_map_instr_consistent_value Hty Hco Hevi Hwfi HunEi).
+      + apply: False_ind. exact: (eval_program_err_ok Hevp).
+  Qed.
+
+  Lemma subst_map_program_consistent_value' E p s1 s2 :
+    well_formed_ssa_program E p ->
+    eval_program E (subst_program (subst_map_program p) p) (OK s1) (OK s2) ->
+    consistent_value (subst_map_program p) s2.
+  Proof.
+    rewrite /subst_map_program. move: (consistent_value_empty s1).
+    move: (consistent_type_empty E).
+    move: (SSAVM.empty atom). elim: p E s1 s2 => [| i p IH] E s1 s2 m Hty Hco Hwf Hev //=.
+    - inversion_clear Hev. move: H => Heq. simpl in Heq. rewrite -Heq. exact: Hco.
+    - rewrite subst_program_cons in Hev.
+      inversion_clear Hev. move: H H0 => Hevi Hevp.
+      move: (well_formed_ssa_hd Hwf) => Hwfi.
+      move: (well_formed_ssa_unchanged_env_hd Hwf) => HunEi.
+      move: (well_formed_ssa_vars_unchanged_hd Hwf) => Hun.
+      move: (ssa_unchanged_program_subset Hun (rvs_instr_subset i)) => {}Hun.
+      rewrite (subst_instr_subst_map_program_rec_unchanged _ Hun) in Hevi Hevp.
+      rewrite (subst_instr_subst_map_instr_unchanged _ (well_formed_ssa_lvs_unchanged_hd Hwf)) in Hevi Hevp.
+      rewrite (consistent_type_instr_succ_typenv _ Hty) in Hevp.
+      case: t Hevi Hevp => [ t |] Hevi Hevp.
+      + apply: (IH _ t _ _ (subst_map_instr_consistent_type Hwfi HunEi Hty)
+                   _ (well_formed_ssa_tl Hwf) Hevp).
+        exact: (subst_map_instr_consistent_value' Hty Hco Hevi Hwfi HunEi).
+      + apply: False_ind. exact: (eval_program_err_ok Hevp).
+  Qed.
+
+
+  (* A combination of consistent_value and consistent_type *)
+
+  Definition consistent_map E m s : Prop :=
+    forall x a, SSAVM.find x m = Some a ->
+                is_defined x E ->
+                are_defined (vars_atom a) E
+                /\ well_typed_atom E a
+                /\ SSATE.vtyp x E = atyp a E
+                /\ (match s with
+                    | OK t => SSAStore.acc x t = eval_atom a t
+                    | ERR => True
+                    end).
+
+  Fixpoint consistent_map_chain E m s p :=
+    match p with
+    | [::] => consistent_map E m s
+    | i::p => consistent_map E m s
+              /\ (forall t, eval_instr E i s t ->
+                            consistent_map_chain (instr_succ_typenv i E) m t p)
+    end.
+
+
+  Lemma consistent_map_chain_consistent E m s p :
+    consistent_map_chain E m s p -> consistent_map E m s.
+  Proof. case: p => [| i p] => //=. tauto. Qed.
+
+
+  Global Instance add_proper_consistent_map_env :
+    Proper (SSATE.Equal ==> eq ==> eq ==> iff) consistent_map.
+  Proof.
+    move=> E1 E2 Heq m1 m2 ? s1 s2 ?; subst. split => Hco x a Hx Hdx.
+    - rewrite -Heq in Hdx *. exact: (Hco _ _ Hx Hdx).
+    - rewrite Heq in Hdx *. exact: (Hco _ _ Hx Hdx).
+  Qed.
+
+  Global Instance add_proper_consistent_map_map :
+    Proper (eq ==> SSAVM.Equal ==> eq ==> iff) consistent_map.
+  Proof.
+    move=> E1 E2 ? m1 m2 Heq s1 s2 ?; subst. split => Hco x a Hx Hdx.
+    - rewrite -Heq in Hx. exact: (Hco _ _ Hx Hdx).
+    - rewrite Heq in Hx. exact: (Hco _ _ Hx Hdx).
+  Qed.
+
+  Global Instance add_proper_consistent_map_state :
+    Proper (eq ==> eq ==> state_equal ==> iff) consistent_map.
+  Proof.
+    move=> E1 E2 ? m1 m2 ? s1 s2 Heq; subst. split => Hco x a Hx Hdx.
+    - move: (Hco _ _ Hx Hdx) => {Hco} H. caseb H. move=> Hdefa Hsma Htyx Hvx.
+      repeat split; try assumption. move: Heq Hvx. case: s1; case: s2 => //=.
+      move=> s1 s2 ->. by apply.
+    - move: (Hco _ _ Hx Hdx) => {Hco} H. caseb H. move=> Hdefa Hsma Htyx Hvx.
+      repeat split; try assumption. move: Heq Hvx. case: s1; case: s2 => //=.
+      move=> s1 s2 ->. by apply.
+  Qed.
+
+  Global Instance add_proper_consistent_map_chain_env :
+    Proper (SSATE.Equal ==> eq ==> eq ==> eq ==> iff) consistent_map_chain.
+  Proof.
+    move=> E1 E2 Heq m1 m2 ? s1 s2 ? p1 p2 ?; subst.
+    elim: p2 E1 E2 m2 s2 Heq => [| i p IH] E1 E2 m s Heq //=.
+    - rewrite Heq. tauto.
+    - move: (add_proper_instr_succ_typenv (Logic.eq_refl i) Heq) => Heq'.
+      split; move => [Hco Hsucc].
+      + split; first by rewrite -Heq. move=> t Hevi. rewrite -Heq in Hevi.
+        move: (IH _ _ m t Heq') => [IH1 IH2]. exact: (IH1 (Hsucc _ Hevi)).
+      + split; first by rewrite Heq. move=> t Hevi. rewrite Heq in Hevi.
+        move: (IH _ _ m t Heq') => [IH1 IH2]. exact: (IH2 (Hsucc _ Hevi)).
+  Qed.
+
+  Global Instance add_proper_consistent_map_chain_map :
+    Proper (eq ==> SSAVM.Equal ==> eq ==> eq ==> iff) consistent_map_chain.
+  Proof.
+    move=> E1 E2 ? m1 m2 Heq s1 s2 ? p1 p2 ?; subst.
+    elim: p2 E2 m1 m2 s2 Heq => [| i p IH] E m1 m2 s Heq //=.
+    - rewrite Heq. tauto.
+    - split; move => [Hco Hsucc].
+      + rewrite Heq in Hco. split; first assumption. move=> t Hevi.
+        apply/(IH _ _ _ _ Heq). exact: (Hsucc _ Hevi).
+      + rewrite -Heq in Hco. split; first assumption. move=> t Hevi.
+        apply/(IH _ _ _ _ Heq). exact: (Hsucc _ Hevi).
+  Qed.
+
+  Global Instance add_proper_consistent_map_chain_state :
+    Proper (eq ==> eq ==> state_equal ==> eq ==> iff) consistent_map_chain.
+  Proof.
+    move=> E1 E2 ? m1 m2 ? s1 s2 Heq p1 p2 ?; subst.
+    elim: p2 E2 m2 s1 s2 Heq => [| i p IH] E m s1 s2 Heq //=.
+    - rewrite Heq. tauto.
+    - split; move => [Hco Hsucc].
+      + split; first by rewrite -Heq. move=> t Hevi.
+        rewrite -Heq in Hevi. exact: (Hsucc _ Hevi).
+      + split; first by rewrite Heq. move=> t Hevi.
+        rewrite Heq in Hevi. exact: (Hsucc _ Hevi).
+  Qed.
+
+
+  Lemma disjoint_consistent_map E m s :
+    VSLemmas.disjoint (TEKS.key_set m) (vars_env E) ->
+    consistent_map E m s.
+  Proof.
+    move=> Hdisj x a Hx Hdx. move: (SSAVM.Lemmas.find_some_mem Hx) => Hmem.
+    move: (TEKS.mem_key_set1 Hmem) => {}Hmem. move: (VSLemmas.mem_disjoint1 Hdisj Hmem).
+    move/memdefP: Hdx. rewrite mem_vars_env. move=> ->. discriminate.
+  Qed.
+
+
+  Lemma consistent_map_eval_eexp E m s e :
+    consistent_map E m (OK s) ->
+    are_defined (vars_eexp e) E ->
+    eval_eexp (subst_eexp m e) E s = eval_eexp e E s.
+  Proof.
+    move=> Hco. elim: e => //=.
+    - move=> v Hwd. rewrite are_defined_singleton in Hwd.
+      dcase (SSAVM.find v m); case => /=.
+      + move=> a. case: a => [ u | ty bs ] /= Hv.
+        * move: (Hco _ _ Hv Hwd) => [Hdefa [Hsma [Htyp Hacc]]].
+          rewrite /acc2z. rewrite Hacc /=. rewrite Htyp /=. reflexivity.
+        * move: (Hco _ _ Hv Hwd) => [Hdefa [Hsma [Htyp Hacc]]].
+          rewrite /acc2z. rewrite Htyp Hacc /=. reflexivity.
+      + reflexivity.
+    - move=> op e IH Hwd. rewrite (IH Hwd). reflexivity.
+    - move=> op e1 IH1 e2 IH2 Hwd. rewrite are_defined_union in Hwd.
+      move/andP: Hwd => [Hwd1 Hwd2]. rewrite (IH1 Hwd1) (IH2 Hwd2). reflexivity.
+    - move=> e IH n Hwd. rewrite (IH Hwd). reflexivity.
+  Qed.
+
+  Lemma consistent_map_eval_rexp E m s e :
+    consistent_map E m (OK s) ->
+    are_defined (vars_rexp e) E ->
+    eval_rexp (subst_rexp m e) s = eval_rexp e s.
+  Proof.
+    move=> Hco. elim: e => //=.
+    - move=> v Hwd. rewrite are_defined_singleton in Hwd.
+      dcase (SSAVM.find v m); case => /=.
+      + move=> a. case: a => [ u | ty bs ] /= Hv.
+        * move: (Hco _ _ Hv Hwd) => [Hdefa [Hsma [Htyp Hacc]]].
+          rewrite /acc2z. rewrite Hacc /=. reflexivity.
+        * move: (Hco _ _ Hv Hwd) => [Hdefa [Hsma [Htyp Hacc]]].
+          rewrite /acc2z. rewrite Hacc /=. reflexivity.
+      + reflexivity.
+    - move=> w op e IH Hwd. rewrite (IH Hwd). reflexivity.
+    - move=> w op e1 IH1 e2 IH2 Hwd. rewrite are_defined_union in Hwd.
+      move/andP: Hwd => [Hwd1 Hwd2]. rewrite (IH1 Hwd1) (IH2 Hwd2). reflexivity.
+    - move=> w e IH n Hwd. rewrite (IH Hwd). reflexivity.
+    - move=> w e IH n Hwd. rewrite (IH Hwd). reflexivity.
+  Qed.
+
+  Lemma consistent_map_eval_eexps E m s es :
+    consistent_map E m (OK s) ->
+    are_defined (vars_eexps es) E ->
+    eval_eexps (subst_eexps m es) E s = eval_eexps es E s.
+  Proof.
+    move=> Hco. elim: es => [| e es IH] //=. rewrite are_defined_union.
+    move/andP=> [Hwde Hwdes]. rewrite subst_eexps_cons /=.
+    rewrite (consistent_map_eval_eexp Hco Hwde) (IH Hwdes). reflexivity.
+  Qed.
+
+  Lemma consistent_map_eval_ebexp E m s e :
+    consistent_map E m (OK s) ->
+    are_defined (vars_ebexp e) E ->
+    eval_ebexp (subst_ebexp m e) E s <-> eval_ebexp e E s.
+  Proof.
+    move=> Hco. elim: e => //=.
+    - move=> e1 e2 Hwd. rewrite are_defined_union in Hwd. move/andP: Hwd => [Hwd1 Hwd2].
+      rewrite (consistent_map_eval_eexp Hco Hwd1) (consistent_map_eval_eexp Hco Hwd2). tauto.
+    - move=> e1 e2 ms Hwd. rewrite !are_defined_union in Hwd.
+      move/andP: Hwd => [Hwd1 /andP [Hwd2 Hwdms]].
+      rewrite (consistent_map_eval_eexp Hco Hwd1) (consistent_map_eval_eexp Hco Hwd2)
+              (consistent_map_eval_eexps Hco Hwdms). tauto.
+    - move=> e1 IH1 e2 IH2 Hwd. rewrite are_defined_union in Hwd.
+      move/andP: Hwd => [Hwd1 Hwd2]. rewrite (IH1 Hwd1) (IH2 Hwd2). tauto.
+  Qed.
+
+  Lemma consistent_map_eval_rbexp E m s e :
+    consistent_map E m (OK s) ->
+    are_defined (vars_rbexp e) E ->
+    eval_rbexp (subst_rbexp m e) s = eval_rbexp e s.
+  Proof.
+    move=> Hco. elim: e => //=.
+    - move=> w e1 e2 Hwd. rewrite are_defined_union in Hwd. move/andP: Hwd => [Hwd1 Hwd2].
+      rewrite (consistent_map_eval_rexp Hco Hwd1) (consistent_map_eval_rexp Hco Hwd2).
+      reflexivity.
+    - move=> w op e1 e2 Hwd. rewrite are_defined_union in Hwd. move/andP: Hwd => [Hwd1 Hwd2].
+      rewrite (consistent_map_eval_rexp Hco Hwd1) (consistent_map_eval_rexp Hco Hwd2).
+      reflexivity.
+    - move=> e IH Hwd. rewrite (IH Hwd). reflexivity.
+    - move=> e1 IH1 e2 IH2 Hwd. rewrite are_defined_union in Hwd. move/andP: Hwd => [Hwd1 Hwd2].
+      rewrite (IH1 Hwd1) (IH2 Hwd2). reflexivity.
+    - move=> e1 IH1 e2 IH2 Hwd. rewrite are_defined_union in Hwd. move/andP: Hwd => [Hwd1 Hwd2].
+      rewrite (IH1 Hwd1) (IH2 Hwd2). reflexivity.
+  Qed.
+
+  Lemma consistent_map_eval_bexp E m s e :
+    consistent_map E m (OK s) ->
+    are_defined (vars_bexp e) E ->
+    eval_bexp (subst_bexp m e) E s <-> eval_bexp e E s.
+  Proof.
+    case: e => [e r] Hco. rewrite /vars_bexp /subst_bexp /eval_bexp /= => Hwd.
+    rewrite are_defined_union in Hwd. move/andP: Hwd => [Hwde Hwdr].
+    rewrite (consistent_map_eval_ebexp Hco Hwde) (consistent_map_eval_rbexp Hco Hwdr).
+    tauto.
+  Qed.
+
+  Lemma consistent_map_atyp E m a s :
+    consistent_map E m s ->
+    are_defined (vars_atom a) E ->
+    atyp (subst_atom m a) E = atyp a E.
+  Proof.
+    move=> Hco. case: a => [ v |] //=. rewrite are_defined_singleton => Hdef.
+    case Hv: (SSAVM.find v m).
+    - rewrite (proj1 (proj2 (proj2 (Hco _ _ Hv Hdef)))). reflexivity.
+    - reflexivity.
+  Qed.
+
+  Lemma consistent_map_eval_atom E m s a :
+    consistent_map E m (OK s) ->
+    are_defined (vars_atom a) E ->
+    eval_atom (subst_atom m a) s = eval_atom a s.
+  Proof.
+    move=> Hco. case: a => [ v |] //=. rewrite are_defined_singleton => Hdef.
+    case Hv: (SSAVM.find v m).
+    - rewrite (proj2 (proj2 (proj2 (Hco _ _ Hv Hdef)))). reflexivity.
+    - reflexivity.
+  Qed.
+
+  Lemma consistent_map_instr_succ_typenv E m s i :
+    consistent_map E m s ->
+    well_formed_instr E i ->
+    SSATE.Equal (instr_succ_typenv (subst_instr m i) E)
+                (instr_succ_typenv i E).
+  Proof.
+    move=> Hco.
+    (case: i => //=); intros;
+      by repeat match goal with
+                | |- SSATE.Equal _ _ => move=> x
+                | H : is_true (well_formed_instr _ _) |- _ =>
+                    move: (well_formed_instr_defined_rvs H) => /= {}H
+                | H : is_true (are_defined (SSAVS.union _ _) _) |- _ =>
+                    let H1 := fresh in
+                    let H2 := fresh in
+                    rewrite are_defined_union in H;
+                    move/andP: H => [H1 H2]
+                | |- context [SSAVM.find ?x (SSATE.add ?t _ _)] =>
+                    let Hxt := fresh in
+                    dcase (x == t); case; intro Hxt;
+                    [ (move/eqP: Hxt => ?); subst; rewrite !(SSATE.Lemmas.find_add_eq (eqxx _))
+                    | (move/negP: Hxt => Hxt); rewrite !(SSATE.Lemmas.find_add_neq Hxt) ]
+                | Hco : consistent_map ?E ?m ?s,
+                    Hdef : is_true (are_defined (vars_atom ?a) ?E)
+                  |- context [atyp (subst_atom ?m ?a) ?E] =>
+                    rewrite (consistent_map_atyp Hco Hdef)
+                | |- ?e = ?e => reflexivity
+                end.
+  Qed.
+
+  Lemma consistent_map_eval_instr E m i s1 s2 :
+    consistent_map E m s1 ->
+    well_formed_instr E i ->
+    eval_instr E (subst_instr m i) s1 s2 <-> eval_instr E i s1 s2.
+  Proof.
+    move=> Hco Hwf. split => Hevi.
+    - (case: i Hevi Hwf Hco => //=); inversion_clear 1; intros;
+      repeat match goal with
+             | |- eval_instr _ _ (ERR SSAStore.t) (ERR SSAStore.t) =>
+                 exact: Eerr
+             | H : is_true (well_formed_instr _ _) |- _ =>
+                 move: (well_formed_instr_defined_rvs Hwf) => /= {}Hwf
+             | H : is_true (are_defined (SSAVS.union _ _) _) |- _ =>
+                 let H1 := fresh in
+                 let H2 := fresh in
+                 rewrite are_defined_union in H;
+                 move/andP: H => [H1 H2]
+             | Hco : consistent_map ?E ?m (OK ?s),
+                 Hdef : is_true (are_defined (vars_atom ?a) ?E),
+                   H : context [eval_atom (subst_atom ?m ?a) ?s] |- _ =>
+                 rewrite (consistent_map_eval_atom Hco Hdef) in H
+             | Hco : consistent_map ?E ?m (OK ?s),
+                 Hdef : is_true (are_defined (vars_bexp ?a) ?E),
+                 H : context [eval_bexp (subst_bexp ?m ?a) ?E ?s] |- _ =>
+                 rewrite (consistent_map_eval_bexp Hco Hdef) in H
+             | Hco : consistent_map ?E ?m (OK ?s),
+                 Hdef : is_true (are_defined (vars_atom ?a) ?E),
+                   H : context [atyp (subst_atom ?m ?a) ?E] |- _ =>
+                 rewrite (consistent_map_atyp Hco Hdef) in H
+             end; eval_instr_intro; assumption.
+    - (case: i Hevi Hwf Hco => //=); inversion_clear 1; intros;
+      repeat match goal with
+             | |- eval_instr _ _ (ERR SSAStore.t) (ERR SSAStore.t) =>
+                 exact: Eerr
+             | H : is_true (well_formed_instr _ _) |- _ =>
+                 move: (well_formed_instr_defined_rvs Hwf) => /= {}Hwf
+             | H : is_true (are_defined (SSAVS.union _ _) _) |- _ =>
+                 let H1 := fresh in
+                 let H2 := fresh in
+                 rewrite are_defined_union in H;
+                 move/andP: H => [H1 H2]
+             end;
+      try match goal with
+          | Hco : consistent_map ?E ?m (OK ?s),
+              Hdef : is_true (are_defined (vars_atom ?a) ?E),
+                H : context [atyp ?a ?E] |- _ =>
+              rewrite -(consistent_map_atyp Hco Hdef) in H
+          end; eval_instr_intro;
+      by repeat match goal with
+                | Hco : consistent_map ?E ?m (OK ?s),
+                    Hdef : is_true (are_defined (vars_atom ?a) ?E)
+                  |- context [eval_atom (subst_atom ?m ?a) ?s] =>
+                    rewrite (consistent_map_eval_atom Hco Hdef)
+                | Hco : consistent_map ?E ?m (OK ?s),
+                    Hdef : is_true (are_defined (vars_bexp ?a) ?E)
+                  |- context [eval_bexp (subst_bexp ?m ?a) ?E ?s] =>
+                    rewrite (consistent_map_eval_bexp Hco Hdef)
+                | H : ?e |- ?e => assumption
+                end.
+  Qed.
+
+  Lemma consistent_map_succ E m i s t :
+    consistent_map E m s ->
+    well_formed_instr E i ->
+    ssa_vars_unchanged_instr (vars_env E) i ->
+    ssa_vars_unchanged_instr (TEKS.key_set m) i ->
+    eval_instr E i s t ->
+    consistent_map (instr_succ_typenv i E) (subst_map_instr m i) t.
+  Proof.
+    move=> Hco Hwf HunEi Hunmi Hev x a Hx Hdefx.
+    case Hunx: (ssa_vars_unchanged_instr (SSAVS.singleton x) i).
+    - rewrite (subst_map_instr_unchanged_find _ Hunx) in Hx.
+      have HdefxE: is_defined x E.
+      { rewrite is_defined_mem_vars_env in Hdefx. rewrite vars_env_instr_succ_typenv in Hdefx.
+        rewrite ssa_unchanged_instr_disjoint_lvs in Hunx. rewrite VSLemmas.mem_union in Hdefx.
+        rewrite VSLemmas.disjoint_singleton_l in Hunx. move/negPf: Hunx => Hunx.
+        rewrite Hunx orbF in Hdefx. rewrite is_defined_mem_vars_env. exact: Hdefx. }
+      move: (Hco _ _ Hx HdefxE) => [Hdefa [Hsma [Htyx Hevx]]].
+      have Huna: ssa_vars_unchanged_instr (vars_atom a) i.
+      { apply: (ssa_unchanged_instr_subset HunEi). apply/defsubP. assumption. }
+      repeat split.
+      + apply: are_defined_instr_succ_typenv. assumption.
+      + rewrite well_typed_atom_unchanged_instr_succ_typenv; first assumption.
+        apply: (ssa_unchanged_instr_subset HunEi). move/defsubP: Hdefa. by apply.
+      + rewrite (vtyp_unchanged_instr_succ_typenv _ Hunx).
+        rewrite (atyp_unchanged_instr_succ_typenv _ Huna). assumption.
+      + move: Hev Hco Hevx. case: t => [ t |] //=. case: s => [ s |] //=.
+        * move=> Hev Hco Hevx.
+          rewrite -(acc_unchanged_instr (ssa_unchanged_instr_singleton1 Hunx) Hev).
+          rewrite -(ssa_unchanged_instr_eval_atom Huna Hev). assumption.
+        * move=> Hev. by inversion Hev.
+    - have Hxm: SSAVM.find x m = None.
+      { apply: SSAVM.Lemmas.not_mem_find_none. apply/negP=> Hmemxm. apply/negPf: Hunx.
+        rewrite ssa_unchanged_instr_singleton ssa_var_unchanged_instr_not_mem.
+        apply/negP=> Hmemxi. rewrite ssa_unchanged_instr_disjoint_lvs in Hunmi.
+        move: (TEKS.mem_key_set1 Hmemxm) => {}Hmemxm.
+        move: (VSLemmas.mem_disjoint1 Hunmi Hmemxm). rewrite Hmemxi. discriminate. }
+      (case: i Hwf HunEi Hunmi Hev Hx Hdefx Hunx => //=); intros;
+      try match goal with
+          | H1 : ?e = None, H2 : ?e = Some _ |- _ =>
+              rewrite H1 in H2; discriminate
+          end.
+      rewrite ssa_unchanged_instr_disjoint_lvs /= in Hunx.
+      rewrite VSLemmas.disjoint_singleton_l in Hunx. move/negPn: Hunx.
+      move/VSLemmas.mem_singleton1 => /eqP ?; subst.
+      rewrite (SSATE.vtyp_add_eq (eqxx _)).
+      case: a0 Hx Hwf HunEi Hunmi Hev Hdefx => [ u | ty bs ] /=  Hx Hwf HunEi Hunmi Hev Hdefx.
+      + case Hu: (SSAVM.find u m) Hx => Hx.
+        * rewrite (SSAVM.Lemmas.find_add_eq (eqxx _)) in Hx. case: Hx => ?; subst.
+          move: (well_formed_instr_defined_rvs Hwf) => /=.
+          rewrite are_defined_singleton => Hdefu.
+          move: (Hco _ _ Hu Hdefu) => [Hdefa [Hsma [Htyu Hevu]]].
+          have Ht0a: ~~ SSAVS.mem t0 (vars_atom a).
+          { rewrite ssa_unchanged_instr_disjoint_lvs /= in HunEi.
+            rewrite VSLemmas.disjoint_singleton_r in HunEi. apply/negP=> Hmemt0.
+            apply/idP: HunEi. move/defsubP: Hdefa => Hsub.
+            exact: (VSLemmas.mem_subset Hmemt0 Hsub). }
+          repeat split.
+          -- apply: are_defined_addr. assumption.
+          -- rewrite well_typed_atom_notin_add; first assumption. exact: Ht0a.
+          -- rewrite (atyp_add_not_mem _ _ Ht0a). assumption.
+          -- move: Hev Hco Hevu. case: t => [ t |] //=. inversion_clear 1.
+             move: H. move=> /= Hev Hco Hevx.
+             rewrite (SSAStore.acc_Upd_eq (eqxx _) Hev). rewrite Hevx.
+             symmetry. apply: (Upd_disjoint_eval_atom Hev).
+             rewrite VSLemmas.disjoint_singleton_l. assumption.
+        * rewrite (SSAVM.Lemmas.find_add_eq (eqxx _)) in Hx. case: Hx => ?; subst.
+          simpl. move: (well_formed_instr_defined_rvs Hwf) => /= Hwd.
+          rewrite ssa_unchanged_instr_disjoint_lvs /= in HunEi.
+          have Hne: u != t0.
+          { move/defsubP: Hwd => Hsub. move: (VSLemmas.disjoint_subset_l HunEi Hsub).
+            rewrite VSLemmas.disjoint_singleton_l. move/VSLemmas.not_mem_singleton1.
+            move/negP => Hne. assumption. }
+          repeat split.
+          -- apply: are_defined_addr. assumption.
+          -- rewrite well_typed_atom_notin_add; first exact: (well_formed_instr_well_typed Hwf).
+             simpl. apply/VSLemmas.not_mem_singleton2. apply/negP. rewrite eq_sym. exact: Hne.
+          -- rewrite (SSATE.vtyp_add_neq Hne). reflexivity.
+          -- move: Hev Hco. case: t => [ t |] //=. move => Hev. inversion_clear Hev.
+             move: H. move=> /= Hev Hco. rewrite (SSAStore.acc_Upd_neq Hne Hev).
+             rewrite (SSAStore.acc_Upd_eq (eqxx _) Hev). reflexivity.
+      + clear Hdefx. rewrite (SSAVM.Lemmas.find_add_eq (eqxx _)) in Hx. case: Hx => ?; subst.
+        simpl. repeat split.
+        * move: (well_formed_instr_well_typed Hwf) => /=. rewrite /well_typed_atom /=.
+          move/andP=> [Hsa Hsbs]. rewrite Hsbs andbT. exact: Hsa.
+        * case: t Hev => [ t |] //=. inversion_clear 1. move: H => /= Hev.
+          rewrite (SSAStore.acc_Upd_eq (eqxx _) Hev). reflexivity.
+  Qed.
+
+  Lemma consistent_map_chain_eval E m p s1 s2 :
+    well_formed_ssa_program E p ->
+    consistent_map_chain E m s1 p ->
+    eval_program E (subst_program m p) s1 s2 <-> eval_program E p s1 s2.
+  Proof.
+    elim: p E m s1 s2 => [| i p IH] E m s1 s2 //=. move=> Hwf [Hco Hcop].
+    move: (well_formed_ssa_hd Hwf) => Hwfi.
+    move: (well_formed_ssa_tl Hwf) => Hwfp.
+    split => Hevp.
+    - rewrite subst_program_cons in Hevp. inversion_clear Hevp.
+      move: H H0 => Hevi Hevp. move/(consistent_map_eval_instr _ Hco Hwfi): Hevi => Hevi.
+      apply: (Econs Hevi). apply/(IH _ _ _ _ Hwfp (Hcop _ Hevi)).
+      rewrite (consistent_map_instr_succ_typenv Hco Hwfi) in Hevp.
+      exact: Hevp.
+    - inversion_clear Hevp. move: H H0 => Hevi Hevp. rewrite subst_program_cons.
+      move: (Hcop _ Hevi) => {}Hcop. move/(consistent_map_eval_instr _ Hco Hwfi): Hevi => Hevi.
+      apply: (Econs Hevi). rewrite (consistent_map_instr_succ_typenv Hco Hwfi).
+      apply/(IH _ _ _ _ (well_formed_ssa_tl Hwf) Hcop). exact: Hevp.
+  Qed.
+
+  Lemma subst_map_program_rec_consistent_map_chain E m s p :
+    well_formed_ssa_program E p ->
+    ssa_vars_unchanged_program (TEKS.key_set m) p ->
+    consistent_map E m s ->
+    consistent_map_chain E (subst_map_program_rec m p) s p.
+  Proof.
+    elim: p E m s => [| i p IH] E m s Hwf Hunmp Hco //=. split.
+    - move=> x a Hx Hdefx. move: (well_formed_ssa_unchanged_env Hwf) => Hun.
+      move: (Hdefx). rewrite -are_defined_singleton. move/defsubP => Hsub.
+      move: (ssa_unchanged_program_subset Hun Hsub) => Hunx.
+      rewrite (subst_map_program_rec_unchanged_find _ (ssa_unchanged_program_tl Hunx)) in Hx.
+      rewrite (subst_map_instr_unchanged_find _ (ssa_unchanged_program_hd Hunx)) in Hx.
+      exact: (Hco _ _ Hx Hdefx).
+    - move=> t Hevi. apply: (IH _ _ _ (well_formed_ssa_tl Hwf)).
+      + apply: (ssa_unchanged_program_subset _ (subst_map_instr_keys_subset _ _)).
+        rewrite ssa_unchanged_program_union. rewrite (ssa_unchanged_program_tl Hunmp) /=.
+        apply: (ssa_unchanged_program_subset _ (lvs_instr_subset _)).
+        exact: (well_formed_ssa_vars_unchanged_hd Hwf).
+      + exact: (consistent_map_succ
+                  Hco (well_formed_ssa_hd Hwf)
+                  (well_formed_ssa_unchanged_env_hd Hwf) (ssa_unchanged_program_hd Hunmp) Hevi).
+  Qed.
+
+  Lemma subst_map_program_consistent_map_chain E s p :
+    well_formed_ssa_program E p ->
+    consistent_map_chain E (subst_map_program p) s p.
+  Proof.
+    move=> Hwf. by apply: (subst_map_program_rec_consistent_map_chain Hwf) => //=.
+  Qed.
+
+
+  Lemma consistent_map_size_of_subst_rexp E m s e :
+    consistent_map E m s ->
+    well_formed_rexp E e ->
+    size_of_rexp (subst_rexp m e) E = size_of_rexp e E.
+  Proof.
+    move=> Hco. elim: e => //=. move=> v. rewrite /well_formed_rexp /=.
+    rewrite are_defined_singleton => /andP [Hdv Hsv].
+    dcase (SSAVM.find v m); case.
+    - move=> a. case: a => /=.
+      + move=> u Hv. move: (Hco _ _ Hv Hdv) => [_ [_ [H _]]].
+        rewrite 2!SSATE.vtyp_vsize. rewrite H. reflexivity.
+      + move=> ty bs Hv. move: (Hco _ _ Hv Hdv) => [_ [_ [H _]]].
+        rewrite SSATE.vtyp_vsize H. reflexivity.
+    - move=> Hv. rewrite /size_of_rexp /=. reflexivity.
+  Qed.
+
+  Lemma consistent_map_disjoint_well_formed_rexp E m s e :
+    consistent_map E m s ->
+    VSLemmas.disjoint (vars_rexp e) (TEKS.key_set m) ->
+    well_formed_rexp E (subst_rexp m e) = well_formed_rexp E e.
+  Proof.
+    move=> Hco. elim: e => //=.
+    - move=> v Hdisj. rewrite VSLemmas.disjoint_singleton_l in Hdisj.
+      rewrite (TEKS.not_mem_key_set_find Hdisj). reflexivity.
+    - move=> w op e IH Hdisj. rewrite /runary.
+      rewrite !well_formed_rexp_runopb. rewrite (IH Hdisj).
+      case Hwf: (well_formed_rexp E e) => //=.
+      rewrite (consistent_map_size_of_subst_rexp Hco Hwf). reflexivity.
+    - move=> w op e1 IH1 e2 IH2. rewrite VSLemmas.disjoint_union_l.
+      move/andP=> [Hdisj1 Hdisj2]. rewrite /rbinary.
+      rewrite !well_formed_rexp_rbinopb. rewrite (IH1 Hdisj1) (IH2 Hdisj2).
+      case Hwf1: (well_formed_rexp E e1) => //=.
+      case Hwf2: (well_formed_rexp E e2) => //=.
+      rewrite (consistent_map_size_of_subst_rexp Hco Hwf1)
+              (consistent_map_size_of_subst_rexp Hco Hwf2). reflexivity.
+    - move=> w e IH n Hdisj. rewrite /ruext. rewrite 2!well_formed_rexp_ruextb /=.
+      rewrite (IH Hdisj). case Hwf: (well_formed_rexp E e) => //=.
+      rewrite (consistent_map_size_of_subst_rexp Hco Hwf). reflexivity.
+    - move=> w e IH n Hdisj. rewrite /rsext. rewrite 2!well_formed_rexp_rsextb /=.
+      rewrite (IH Hdisj). case Hwf: (well_formed_rexp E e) => //=.
+      rewrite (consistent_map_size_of_subst_rexp Hco Hwf). reflexivity.
+  Qed.
+
+  Lemma consistent_map_disjoint_well_formed_rbexp E m s e :
+    consistent_map E m s ->
+    VSLemmas.disjoint (vars_rbexp e) (TEKS.key_set m) ->
+    well_formed_rbexp E (subst_rbexp m e) = well_formed_rbexp E e.
+  Proof.
+    move=> Hco. elim: e => //=.
+    - move=> w e1 e2. rewrite VSLemmas.disjoint_union_l => /andP [Hdisj1 Hdisj2].
+      rewrite 2!well_formed_rbexp_reqb.
+      rewrite (consistent_map_disjoint_well_formed_rexp Hco Hdisj1)
+              (consistent_map_disjoint_well_formed_rexp Hco Hdisj2).
+      case Hwf1: (well_formed_rexp E e1) => //=. case Hwf2: (well_formed_rexp E e2) => //=.
+      rewrite (consistent_map_size_of_subst_rexp Hco Hwf1)
+              (consistent_map_size_of_subst_rexp Hco Hwf2). reflexivity.
+    - move=> w op e1 e2. rewrite VSLemmas.disjoint_union_l => /andP [Hdisj1 Hdisj2].
+      rewrite 2!well_formed_rbexp_rcmpb.
+      rewrite (consistent_map_disjoint_well_formed_rexp Hco Hdisj1)
+              (consistent_map_disjoint_well_formed_rexp Hco Hdisj2).
+      case Hwf1: (well_formed_rexp E e1) => //=. case Hwf2: (well_formed_rexp E e2) => //=.
+      rewrite (consistent_map_size_of_subst_rexp Hco Hwf1)
+              (consistent_map_size_of_subst_rexp Hco Hwf2). reflexivity.
+    - move=> e1 IH1 e2 IH2. rewrite VSLemmas.disjoint_union_l => /andP [Hdisj1 Hdisj2].
+      rewrite 2!well_formed_rbexp_randb. rewrite (IH1 Hdisj1) (IH2 Hdisj2).
+      reflexivity.
+    - move=> e1 IH1 e2 IH2. rewrite VSLemmas.disjoint_union_l => /andP [Hdisj1 Hdisj2].
+      rewrite 2!well_formed_rbexp_rorb. rewrite (IH1 Hdisj1) (IH2 Hdisj2).
+      reflexivity.
+  Qed.
+
+  Lemma consistent_map_disjoint_well_formed_bexp E m s e :
+    consistent_map E m s ->
+    VSLemmas.disjoint (vars_bexp e) (TEKS.key_set m) ->
+    well_formed_bexp E (subst_bexp m e) = well_formed_bexp E e.
+  Proof.
+    move=> Hco. case: e => [e r]. rewrite /vars_bexp /=.
+    rewrite VSLemmas.disjoint_union_l => /andP [Hdisje Hdisjr].
+    rewrite /subst_bexp 2!well_formed_bexp_split /=.
+    rewrite (disjoint_well_formed_ebexp _ Hdisje)
+            (consistent_map_disjoint_well_formed_rbexp Hco Hdisjr).
+    reflexivity.
+  Qed.
+
+
+  (* A chain of consistent types *)
+
+  Definition weak_consistent_type (m : SSAVM.t atom) (E : SSATE.env) : Prop :=
+    forall x a, SSAVM.find x m = Some a ->
+                is_defined x E ->
+                are_defined (vars_atom a) E
+                /\ well_typed_atom E a
+                /\ SSATE.vtyp x E = atyp a E.
+
+  Fixpoint weak_consistent_type_chain E m p :=
+    match p with
+    | [::] => weak_consistent_type m E
+    | i::p => weak_consistent_type m E
+              /\ weak_consistent_type_chain (instr_succ_typenv i E) m p
+    end.
+
+
+  Lemma consistent_map_weak_type E m s :
+    consistent_map E m s -> weak_consistent_type m E.
+  Proof. move=> Hco x a Hx Hdx. move: (Hco _ _ Hx Hdx). tauto. Qed.
+
+  Lemma consistent_value_weak_type_map E m s :
+    consistent_value m s -> weak_consistent_type m E ->
+    consistent_map E m (OK s).
+  Proof. move=> Hev Hty x a Hx Hdx. move: (Hev _ _ Hx) (Hty _ _ Hx Hdx). tauto. Qed.
+
+  Lemma consistent_type_weak m E :
+    consistent_type m E -> weak_consistent_type m E.
+  Proof. move=> Hco x a Hx Hdx. move: (Hco _ _ Hx). tauto. Qed.
+
+  Lemma consistent_value_type_map E m s :
+    consistent_value m s -> consistent_type m E ->
+    consistent_map E m (OK s).
+  Proof.
+    move=> Hev Hty.
+    exact: (consistent_value_weak_type_map Hev (consistent_type_weak Hty)).
+  Qed.
+
+  Lemma weak_consistent_type_chain_consistent E m p :
+    weak_consistent_type_chain E m p -> weak_consistent_type m E.
+  Proof. case: p => [| i p] => //=. tauto. Qed.
+
+
+  Global Instance add_proper_weak_consistent_type_map :
+    Proper (SSAVM.Equal ==> eq ==> iff) weak_consistent_type.
+  Proof.
+    move=> m1 m2 Heq s1 s2 ?; subst. split => Hco x a Hx Hdx.
+    - rewrite -Heq in Hx. exact: (Hco _ _ Hx Hdx).
+    - rewrite Heq in Hx. exact: (Hco _ _ Hx Hdx).
+  Qed.
+
+  Global Instance add_proper_weak_consistent_type_env :
+    Proper (eq ==> SSATE.Equal ==> iff) weak_consistent_type.
+  Proof.
+    move=> m1 m2 ? E1 E2 Heq; subst. split => Hco x a Hx Hdx.
+    - move: (Hco _ _ Hx). rewrite Heq. tauto.
+    - move: (Hco _ _ Hx). rewrite -Heq. tauto.
+  Qed.
+
+  Global Instance add_proper_weak_consistent_type_chain_env :
+    Proper (SSATE.Equal ==> eq ==> eq ==> iff) weak_consistent_type_chain.
+  Proof.
+    move=> E1 E2 Heq m1 m2 ? p1 p2 ?; subst.
+    elim: p2 E1 E2 m2 Heq => [| i p IH] E1 E2 m Heq //=.
+    - rewrite Heq. tauto.
+    - move: (add_proper_instr_succ_typenv (Logic.eq_refl i) Heq) => Heq'.
+      split; move => [Hco Hsucc].
+      + split; first by rewrite -Heq. apply/(IH _ _ m Heq'). exact: Hsucc.
+      + split; first by rewrite Heq. apply/(IH _ _ m Heq'). exact: Hsucc.
+  Qed.
+
+  Global Instance add_proper_weak_consistent_type_chain_map :
+    Proper (eq ==> SSAVM.Equal ==> eq ==> iff) weak_consistent_type_chain.
+  Proof.
+    move=> E1 E2 ? m1 m2 Heq p1 p2 ?; subst.
+    elim: p2 E2 m1 m2 Heq => [| i p IH] E m1 m2 Heq //=.
+    - rewrite Heq. tauto.
+    - split; move => [Hco Hsucc].
+      + rewrite Heq in Hco. split; first assumption. apply/(IH _ _ _ Heq). exact: Hsucc.
+      + rewrite -Heq in Hco. split; first assumption. apply/(IH _ _ _ Heq). exact: Hsucc.
+  Qed.
+
+
+  Lemma disjoint_weak_consistent_type E m :
+    VSLemmas.disjoint (TEKS.key_set m) (vars_env E) ->
+    weak_consistent_type m E.
+  Proof.
+    move=> Hdisj x a Hx Hdx. move: (SSAVM.Lemmas.find_some_mem Hx) => Hmem.
+    move: (TEKS.mem_key_set1 Hmem) => {}Hmem. move: (VSLemmas.mem_disjoint1 Hdisj Hmem).
+    move/memdefP: Hdx. rewrite mem_vars_env. move=> ->. discriminate.
+  Qed.
+
+  Lemma weak_consistent_type_empty E : weak_consistent_type (SSAVM.empty _) E.
+  Proof.
+    move=> x a Hx. rewrite SSAVM.Lemmas.empty_o in Hx. discriminate.
+  Qed.
+
+  Lemma weak_consistent_type_atyp E m a :
+    weak_consistent_type m E ->
+    are_defined (vars_atom a) E ->
+    atyp (subst_atom m a) E = atyp a E.
+  Proof.
+    move=> Hco. case: a => //=. move=> v. rewrite are_defined_singleton => Hdv.
+    case Hv: (SSAVM.find v m) => //=. move: (proj2 (proj2 (Hco _ _ Hv Hdv))).
+    symmetry. assumption.
+  Qed.
+
+  Lemma weak_consistent_type_asize E m a :
+    weak_consistent_type m E ->
+    are_defined (vars_atom a) E ->
+    asize (subst_atom m a) E = asize a E.
+  Proof.
+    move=> Hco Hdef. rewrite /asize. rewrite (weak_consistent_type_atyp Hco Hdef). reflexivity.
+  Qed.
+
+  Lemma weak_consistent_type_size_of_subst_rexp E m e :
+    weak_consistent_type m E ->
+    well_formed_rexp E e ->
+    size_of_rexp (subst_rexp m e) E = size_of_rexp e E.
+  Proof.
+    move=> Hco. elim: e => //=. move=> v. rewrite /well_formed_rexp /=.
+    rewrite are_defined_singleton => /andP [Hdv Hsv].
+    dcase (SSAVM.find v m); case.
+    - move=> a. case: a => /=.
+      + move=> u Hv. move: (Hco _ _ Hv Hdv) => [_ [_ H]].
+        rewrite 2!SSATE.vtyp_vsize. rewrite H. reflexivity.
+      + move=> ty bs Hv. move: (Hco _ _ Hv Hdv) => [_ [_ H]].
+        rewrite SSATE.vtyp_vsize H. reflexivity.
+    - move=> Hv. rewrite /size_of_rexp /=. reflexivity.
+  Qed.
+
+  Lemma weak_consistent_type_disjoint_well_formed_rexp E m e :
+    weak_consistent_type m E ->
+    VSLemmas.disjoint (vars_rexp e) (TEKS.key_set m) ->
+    well_formed_rexp E (subst_rexp m e) = well_formed_rexp E e.
+  Proof.
+    move=> Hco. elim: e => //=.
+    - move=> v Hdisj. rewrite VSLemmas.disjoint_singleton_l in Hdisj.
+      rewrite (TEKS.not_mem_key_set_find Hdisj). reflexivity.
+    - move=> w op e IH Hdisj. rewrite /runary.
+      rewrite !well_formed_rexp_runopb. rewrite (IH Hdisj).
+      case Hwf: (well_formed_rexp E e) => //=.
+      rewrite (weak_consistent_type_size_of_subst_rexp Hco Hwf). reflexivity.
+    - move=> w op e1 IH1 e2 IH2. rewrite VSLemmas.disjoint_union_l.
+      move/andP=> [Hdisj1 Hdisj2]. rewrite /rbinary.
+      rewrite !well_formed_rexp_rbinopb. rewrite (IH1 Hdisj1) (IH2 Hdisj2).
+      case Hwf1: (well_formed_rexp E e1) => //=.
+      case Hwf2: (well_formed_rexp E e2) => //=.
+      rewrite (weak_consistent_type_size_of_subst_rexp Hco Hwf1)
+              (weak_consistent_type_size_of_subst_rexp Hco Hwf2). reflexivity.
+    - move=> w e IH n Hdisj. rewrite /ruext. rewrite 2!well_formed_rexp_ruextb /=.
+      rewrite (IH Hdisj). case Hwf: (well_formed_rexp E e) => //=.
+      rewrite (weak_consistent_type_size_of_subst_rexp Hco Hwf). reflexivity.
+    - move=> w e IH n Hdisj. rewrite /rsext. rewrite 2!well_formed_rexp_rsextb /=.
+      rewrite (IH Hdisj). case Hwf: (well_formed_rexp E e) => //=.
+      rewrite (weak_consistent_type_size_of_subst_rexp Hco Hwf). reflexivity.
+  Qed.
+
+  Lemma weak_consistent_type_disjoint_well_formed_rbexp E m e :
+    weak_consistent_type m E ->
+    VSLemmas.disjoint (vars_rbexp e) (TEKS.key_set m) ->
+    well_formed_rbexp E (subst_rbexp m e) = well_formed_rbexp E e.
+  Proof.
+    move=> Hco. elim: e => //=.
+    - move=> w e1 e2. rewrite VSLemmas.disjoint_union_l => /andP [Hdisj1 Hdisj2].
+      rewrite 2!well_formed_rbexp_reqb.
+      rewrite (weak_consistent_type_disjoint_well_formed_rexp Hco Hdisj1)
+              (weak_consistent_type_disjoint_well_formed_rexp Hco Hdisj2).
+      case Hwf1: (well_formed_rexp E e1) => //=. case Hwf2: (well_formed_rexp E e2) => //=.
+      rewrite (weak_consistent_type_size_of_subst_rexp Hco Hwf1)
+              (weak_consistent_type_size_of_subst_rexp Hco Hwf2). reflexivity.
+    - move=> w op e1 e2. rewrite VSLemmas.disjoint_union_l => /andP [Hdisj1 Hdisj2].
+      rewrite 2!well_formed_rbexp_rcmpb.
+      rewrite (weak_consistent_type_disjoint_well_formed_rexp Hco Hdisj1)
+              (weak_consistent_type_disjoint_well_formed_rexp Hco Hdisj2).
+      case Hwf1: (well_formed_rexp E e1) => //=. case Hwf2: (well_formed_rexp E e2) => //=.
+      rewrite (weak_consistent_type_size_of_subst_rexp Hco Hwf1)
+              (weak_consistent_type_size_of_subst_rexp Hco Hwf2). reflexivity.
+    - move=> e1 IH1 e2 IH2. rewrite VSLemmas.disjoint_union_l => /andP [Hdisj1 Hdisj2].
+      rewrite 2!well_formed_rbexp_randb. rewrite (IH1 Hdisj1) (IH2 Hdisj2).
+      reflexivity.
+    - move=> e1 IH1 e2 IH2. rewrite VSLemmas.disjoint_union_l => /andP [Hdisj1 Hdisj2].
+      rewrite 2!well_formed_rbexp_rorb. rewrite (IH1 Hdisj1) (IH2 Hdisj2).
+      reflexivity.
+  Qed.
+
+  Lemma weak_consistent_type_disjoint_well_formed_bexp E m e :
+    weak_consistent_type m E ->
+    VSLemmas.disjoint (vars_bexp e) (TEKS.key_set m) ->
+    well_formed_bexp E (subst_bexp m e) = well_formed_bexp E e.
+  Proof.
+    move=> Hco. case: e => [e r]. rewrite /vars_bexp /=.
+    rewrite VSLemmas.disjoint_union_l => /andP [Hdisje Hdisjr].
+    rewrite /subst_bexp 2!well_formed_bexp_split /=.
+    rewrite (disjoint_well_formed_ebexp _ Hdisje)
+            (weak_consistent_type_disjoint_well_formed_rbexp Hco Hdisjr).
+    reflexivity.
+  Qed.
+
+
+  Lemma weak_consistent_type_instr_succ_typenv E m i :
+    weak_consistent_type m E ->
+    well_formed_instr E i ->
+    SSATE.Equal (instr_succ_typenv (subst_instr m i) E)
+                (instr_succ_typenv i E).
+  Proof.
+    move=> Hco.
+    (case: i => //=); intros;
+      by repeat match goal with
+                | |- SSATE.Equal _ _ => move=> x
+                | H : is_true (well_formed_instr _ _) |- _ =>
+                    move: (well_formed_instr_defined_rvs H) => /= {}H
+                | H : is_true (are_defined (SSAVS.union _ _) _) |- _ =>
+                    let H1 := fresh in
+                    let H2 := fresh in
+                    rewrite are_defined_union in H;
+                    move/andP: H => [H1 H2]
+                | |- context [SSAVM.find ?x (SSATE.add ?t _ _)] =>
+                    let Hxt := fresh in
+                    dcase (x == t); case; intro Hxt;
+                    [ (move/eqP: Hxt => ?); subst; rewrite !(SSATE.Lemmas.find_add_eq (eqxx _))
+                    | (move/negP: Hxt => Hxt); rewrite !(SSATE.Lemmas.find_add_neq Hxt) ]
+                | Hco : weak_consistent_type ?m ?E,
+                    Hdef : is_true (are_defined (vars_atom ?a) ?E)
+                  |- context [atyp (subst_atom ?m ?a) ?E] =>
+                    rewrite (weak_consistent_type_atyp Hco Hdef)
+                | |- ?e = ?e => reflexivity
+             end.
+  Qed.
+
+  Lemma weak_consistent_type_succ E m i :
+    weak_consistent_type m E ->
+    well_formed_instr E i ->
+    ssa_vars_unchanged_instr (vars_env E) i ->
+    ssa_vars_unchanged_instr (TEKS.key_set m) i ->
+    weak_consistent_type (subst_map_instr m i) (instr_succ_typenv i E).
+  Proof.
+    move=> Hco Hwf HunEi Hunmi x a Hx Hdefx.
+    case Hunx: (ssa_vars_unchanged_instr (SSAVS.singleton x) i).
+    - rewrite (subst_map_instr_unchanged_find _ Hunx) in Hx.
+      have HdefxE: is_defined x E.
+      { rewrite is_defined_mem_vars_env in Hdefx. rewrite vars_env_instr_succ_typenv in Hdefx.
+        rewrite ssa_unchanged_instr_disjoint_lvs in Hunx. rewrite VSLemmas.mem_union in Hdefx.
+        rewrite VSLemmas.disjoint_singleton_l in Hunx. move/negPf: Hunx => Hunx.
+        rewrite Hunx orbF in Hdefx. rewrite is_defined_mem_vars_env. exact: Hdefx. }
+      move: (Hco _ _ Hx HdefxE) => [Hdefa [Hsma Htyx]].
+      have Huna: ssa_vars_unchanged_instr (vars_atom a) i.
+      { apply: (ssa_unchanged_instr_subset HunEi). apply/defsubP. assumption. }
+      repeat split.
+      + apply: are_defined_instr_succ_typenv. assumption.
+      + rewrite well_typed_atom_unchanged_instr_succ_typenv; first assumption.
+        apply: (ssa_unchanged_instr_subset HunEi). move/defsubP: Hdefa. by apply.
+      + rewrite (vtyp_unchanged_instr_succ_typenv _ Hunx).
+        rewrite (atyp_unchanged_instr_succ_typenv _ Huna). assumption.
+    - have Hxm: SSAVM.find x m = None.
+      { apply: SSAVM.Lemmas.not_mem_find_none. apply/negP=> Hmemxm. apply/negPf: Hunx.
+        rewrite ssa_unchanged_instr_singleton ssa_var_unchanged_instr_not_mem.
+        apply/negP=> Hmemxi. rewrite ssa_unchanged_instr_disjoint_lvs in Hunmi.
+        move: (TEKS.mem_key_set1 Hmemxm) => {}Hmemxm.
+        move: (VSLemmas.mem_disjoint1 Hunmi Hmemxm). rewrite Hmemxi. discriminate. }
+      (case: i Hwf HunEi Hunmi Hx Hdefx Hunx => //=); intros;
+      try match goal with
+          | H1 : ?e = None, H2 : ?e = Some _ |- _ =>
+              rewrite H1 in H2; discriminate
+          end.
+      rewrite ssa_unchanged_instr_disjoint_lvs /= in Hunx.
+      rewrite VSLemmas.disjoint_singleton_l in Hunx. move/negPn: Hunx.
+      move/VSLemmas.mem_singleton1 => /eqP ?; subst.
+      rewrite (SSATE.vtyp_add_eq (eqxx _)).
+      case: a0 Hx Hwf HunEi Hunmi Hdefx => [ u | ty bs ] /=  Hx Hwf HunEi Hunmi Hdefx.
+      + case Hu: (SSAVM.find u m) Hx => Hx.
+        * rewrite (SSAVM.Lemmas.find_add_eq (eqxx _)) in Hx. case: Hx => ?; subst.
+          move: (well_formed_instr_defined_rvs Hwf) => /=.
+          rewrite are_defined_singleton => Hdefu.
+          move: (Hco _ _ Hu Hdefu) => [Hdefa [Hsma Htyu]].
+          have Hta: ~~ SSAVS.mem t (vars_atom a).
+          { rewrite ssa_unchanged_instr_disjoint_lvs /= in HunEi.
+            rewrite VSLemmas.disjoint_singleton_r in HunEi. apply/negP=> Hmemt.
+            apply/idP: HunEi. move/defsubP: Hdefa => Hsub.
+            exact: (VSLemmas.mem_subset Hmemt Hsub). }
+          repeat split.
+          -- apply: are_defined_addr. assumption.
+          -- rewrite well_typed_atom_notin_add; first assumption.
+             exact: Hta.
+          -- rewrite (atyp_add_not_mem _ _ Hta). assumption.
+        * rewrite (SSAVM.Lemmas.find_add_eq (eqxx _)) in Hx. case: Hx => ?; subst.
+          simpl. move: (well_formed_instr_defined_rvs Hwf) => /= Hwd.
+          rewrite ssa_unchanged_instr_disjoint_lvs /= in HunEi.
+          have Hne: u != t.
+          { move/defsubP: Hwd => Hsub. move: (VSLemmas.disjoint_subset_l HunEi Hsub).
+            rewrite VSLemmas.disjoint_singleton_l. move/VSLemmas.not_mem_singleton1.
+            move/negP => Hne. assumption. }
+          repeat split.
+          -- apply: are_defined_addr. assumption.
+          -- rewrite well_typed_atom_notin_add; first exact: (well_formed_instr_well_typed Hwf).
+             simpl. apply/VSLemmas.not_mem_singleton2. apply/negP. rewrite eq_sym. exact: Hne.
+          -- rewrite (SSATE.vtyp_add_neq Hne). reflexivity.
+      + clear Hdefx. rewrite (SSAVM.Lemmas.find_add_eq (eqxx _)) in Hx. case: Hx => ?; subst.
+        simpl. repeat split.
+        move: (well_formed_instr_well_typed Hwf) => /=. rewrite /well_typed_atom /=.
+        move/andP=> [Hsa Hsbs]. rewrite Hsbs andbT. exact: Hsa.
+  Qed.
+
+  Lemma subst_map_program_rec_weak_consistent_type_chain E m p :
+    well_formed_ssa_program E p ->
+    ssa_vars_unchanged_program (TEKS.key_set m) p ->
+    weak_consistent_type m E ->
+    weak_consistent_type_chain E (subst_map_program_rec m p) p.
+  Proof.
+    elim: p E m => [| i p IH] E m Hwf Hunmp Hco //=. split.
+    - move=> x a Hx Hdefx. move: (well_formed_ssa_unchanged_env Hwf) => Hun.
+      move: (Hdefx). rewrite -are_defined_singleton. move/defsubP => Hsub.
+      move: (ssa_unchanged_program_subset Hun Hsub) => Hunx.
+      rewrite (subst_map_program_rec_unchanged_find _ (ssa_unchanged_program_tl Hunx)) in Hx.
+      rewrite (subst_map_instr_unchanged_find _ (ssa_unchanged_program_hd Hunx)) in Hx.
+      exact: (Hco _ _ Hx Hdefx).
+    - apply: (IH _ _ (well_formed_ssa_tl Hwf)).
+      + apply: (ssa_unchanged_program_subset _ (subst_map_instr_keys_subset _ _)).
+        rewrite ssa_unchanged_program_union. rewrite (ssa_unchanged_program_tl Hunmp) /=.
+        apply: (ssa_unchanged_program_subset _ (lvs_instr_subset _)).
+        exact: (well_formed_ssa_vars_unchanged_hd Hwf).
+      + exact: (weak_consistent_type_succ
+                  Hco (well_formed_ssa_hd Hwf)
+                  (well_formed_ssa_unchanged_env_hd Hwf) (ssa_unchanged_program_hd Hunmp)).
+  Qed.
+
+  Lemma subst_map_program_weak_consistent_type_chain E p :
+    well_formed_ssa_program E p ->
+    weak_consistent_type_chain E (subst_map_program p) p.
+  Proof.
+    move=> Hwf. by apply: (subst_map_program_rec_weak_consistent_type_chain Hwf) => //=.
+  Qed.
+
+
+  (* Initial *)
+
+  Lemma subst_map_program_consistent_map_init E s p :
+    well_formed_ssa_program E p ->
+    consistent_map E (subst_map_program p) s.
+  Proof.
+    move=> Hwf. apply: disjoint_consistent_map.
+    exact: subst_map_program_keys_disjoint.
+  Qed.
+
+  Lemma subst_map_program_weak_consistent_type_init E p :
+    well_formed_ssa_program E p ->
+    weak_consistent_type (subst_map_program p) E.
+  Proof.
+    move=> Hwf. apply: disjoint_weak_consistent_type.
+    exact: subst_map_program_keys_disjoint.
+  Qed.
+
+
+  (* Evaluation of substituted programs *)
+
+  Lemma subst_map_program_eval E p s1 s2 :
+    well_formed_ssa_program E p ->
+    eval_program E (subst_program (subst_map_program p) p) s1 s2 <->
+      eval_program E p s1 s2.
+  Proof.
+    move=> Hwf. apply: (consistent_map_chain_eval _ Hwf).
+    exact: subst_map_program_consistent_map_chain.
+  Qed.
+
+
+  (* Soundness and completeness *)
+
+  Lemma rewrite_mov_sound s :
+    well_formed_ssa_spec s ->
+    valid_spec (rewrite_mov s) -> valid_spec s.
+  Proof.
+    case: s => E f p g. rewrite /well_formed_ssa_spec /well_formed_spec => /= H.
+    caseb H. move=> Hwff Hwfp Hwfg HunEp Hssap.
+    rewrite /valid_spec /valid_spec_ok /valid_spec_err /rewrite_mov /subst_map_spec /=.
+    move=> [Hok Herr].
+    have Hwfssap: well_formed_ssa_program E p.
+    { rewrite /well_formed_ssa_program. by rewrite Hwfp HunEp Hssap. }
+    split.
+    - move=> s1 s2 Hco Hevf Hevp.
+      have Hevf': eval_bexp (subst_bexp (subst_map_program p) f) E s1.
+      { rewrite disjoint_subst_bexp; first exact: Hevf.
+        apply: (SSAVS.Lemmas.disjoint_subset_l _ (subst_map_program_keys_subset p)).
+        apply: (SSAVS.Lemmas.disjoint_subset_r _ (well_formed_bexp_vars_subset Hwff)).
+        rewrite SSAVS.Lemmas.disjoint_sym.
+        rewrite ssa_unchanged_program_disjoint_lvs in HunEp.
+        exact: HunEp. }
+      have Hevp': eval_program E (subst_program (subst_map_program p) p) (OK s1) (OK s2).
+      { apply/(subst_map_program_eval _ _ Hwfssap). exact: Hevp. }
+      move: (Hok s1 s2 Hco Hevf' Hevp'). rewrite (subst_map_program_succ_typenv Hwfssap).
+      move/(subst_bexp_eval_unchanged
+              _
+              (subst_map_program_consistent_value Hwfssap Hevp)
+              (subst_map_program_consistent_type Hwfssap)). by apply.
+    - move=> s Hco Hevf Hevp.
+      have Hevf': eval_bexp (subst_bexp (subst_map_program p) f) E s.
+      { rewrite disjoint_subst_bexp; first exact: Hevf.
+        apply: (SSAVS.Lemmas.disjoint_subset_l _ (subst_map_program_keys_subset p)).
+        apply: (SSAVS.Lemmas.disjoint_subset_r _ (well_formed_bexp_vars_subset Hwff)).
+        rewrite SSAVS.Lemmas.disjoint_sym.
+        rewrite ssa_unchanged_program_disjoint_lvs in HunEp.
+        exact: HunEp. }
+      apply: (Herr _ Hco Hevf'). apply/(subst_map_program_eval _ _ Hwfssap).
+      exact: Hevp.
+  Qed.
+
+  Lemma rewrite_mov_complete s :
+    well_formed_ssa_spec s ->
+    valid_spec s -> valid_spec (rewrite_mov s).
+  Proof.
+    case: s => E f p g. rewrite /well_formed_ssa_spec /well_formed_spec => /= H.
+    caseb H. move=> Hwff Hwfp Hwfg HunEp Hssap.
+    rewrite /valid_spec /valid_spec_ok /valid_spec_err /rewrite_mov /subst_map_spec /=.
+    move=> [Hok Herr].
+    have Hwfssap: well_formed_ssa_program E p.
+    { rewrite /well_formed_ssa_program. by rewrite Hwfp HunEp Hssap. }
+    split.
+    - move=> s1 s2 Hco Hevf Hevp.
+      have Hevf': eval_bexp f E s1.
+      { rewrite disjoint_subst_bexp in Hevf; first exact: Hevf.
+        apply: (SSAVS.Lemmas.disjoint_subset_l _ (subst_map_program_keys_subset p)).
+        apply: (SSAVS.Lemmas.disjoint_subset_r _ (well_formed_bexp_vars_subset Hwff)).
+        rewrite SSAVS.Lemmas.disjoint_sym.
+        rewrite ssa_unchanged_program_disjoint_lvs in HunEp.
+        exact: HunEp. }
+      have Hevp': eval_program E p (OK s1) (OK s2).
+      { move/(subst_map_program_eval _ _ Hwfssap) : Hevp. by apply. }
+      move: (Hok s1 s2 Hco Hevf' Hevp'). rewrite (subst_map_program_succ_typenv Hwfssap).
+      move/(subst_bexp_eval_unchanged
+              _
+              (subst_map_program_consistent_value Hwfssap Hevp')
+              (subst_map_program_consistent_type Hwfssap)). by apply.
+    - move=> s Hco Hevf Hevp.
+      have Hevf': eval_bexp f E s.
+      { rewrite disjoint_subst_bexp in Hevf; first exact: Hevf.
+        apply: (SSAVS.Lemmas.disjoint_subset_l _ (subst_map_program_keys_subset p)).
+        apply: (SSAVS.Lemmas.disjoint_subset_r _ (well_formed_bexp_vars_subset Hwff)).
+        rewrite SSAVS.Lemmas.disjoint_sym.
+        rewrite ssa_unchanged_program_disjoint_lvs in HunEp.
+        exact: HunEp. }
+      apply: (Herr _ Hco Hevf'). move/(subst_map_program_eval _ _ Hwfssap) : Hevp.
+      by apply.
+  Qed.
+
+
+  (* well-formedness *)
+
+  Lemma weak_consistent_type_are_defined_atom E m a :
+    weak_consistent_type m E ->
+    are_defined (vars_atom a) E ->
+    are_defined (vars_atom (subst_atom m a)) E.
+  Proof.
+    case: a => [ v | ty bs ] //= Hco Hdv. rewrite are_defined_singleton in Hdv.
+    case Hv: (SSAVM.find v m).
+    - move: (Hco _ _ Hv Hdv). tauto.
+    - simpl. rewrite are_defined_singleton. assumption.
+  Qed.
+
+  Lemma weak_consistent_type_well_typed_atom E m a :
+    weak_consistent_type m E ->
+    are_defined (vars_atom a) E ->
+    well_typed_atom E a ->
+    well_typed_atom E (subst_atom m a).
+  Proof.
+    case: a => [ v | ty bs ] //= Hco Hdv Hwt. rewrite are_defined_singleton in Hdv.
+    rewrite /well_typed_atom /= in Hwt *. case Hv: (SSAVM.find v m).
+    - move: (Hco _ _ Hv Hdv) => [Hda [Hwta Htyv]]. exact: Hwta.
+    - simpl. exact: Hwt.
+  Qed.
+
+  Lemma well_typed_eexp_of_atom E a :
+    well_typed_atom E a ->
+    well_typed_eexp E (eexp_of_atom a).
+  Proof. by case: a => [ v | ty bs ] //=. Qed.
+
+  Lemma well_typed_rexp_of_atom E a :
+    well_typed_atom E a ->
+    well_typed_rexp E (rexp_of_atom a).
+  Proof.
+    case: a => [ v | ty bs ] //=.
+    - rewrite /well_typed_atom /=. rewrite andbT /well_sized_atom /=.
+      case: (is_unsigned (SSATE.vtyp v E)) => //=.
+      move=> H. apply: (ltn_trans _ H). done.
+    - rewrite /well_typed_atom /= /well_sized_atom. move/andP=> /= [H ->]. rewrite andbT.
+      case: (is_unsigned ty) H => //=.
+      move=> H. apply: (ltn_trans _ H). done.
+  Qed.
+
+  Lemma subst_eexp_are_defined E m e :
+    weak_consistent_type m E ->
+    are_defined (vars_eexp e) E ->
+    are_defined (vars_eexp (subst_eexp m e)) E.
+  Proof.
+    move=> Hco. elim: e => //=.
+    - move=> v. rewrite are_defined_singleton /= => Hdv.
+      case Hv: (SSAVM.find v m).
+      + move: (Hco _ _ Hv Hdv) => [Hda [Hwta Htyv]]. rewrite vars_eexp_of_atom.
+        exact: Hda.
+      + simpl. rewrite are_defined_singleton. exact: Hdv.
+    - move=> op e1 IH1 e2 IH2. rewrite 2!are_defined_union.
+      move/andP=> [Hdef1 Hdef2]. rewrite (IH1 Hdef1) (IH2 Hdef2). reflexivity.
+  Qed.
+
+  Lemma subst_eexp_well_typed E m e :
+    weak_consistent_type m E ->
+    are_defined (vars_eexp e) E ->
+    well_typed_eexp E e ->
+    well_typed_eexp E (subst_eexp m e).
+  Proof.
+    move=> Hco. elim: e => //=.
+    - move=> v Hdv _. rewrite are_defined_singleton in Hdv.
+      case Hv: (SSAVM.find v m).
+      + move: (Hco _ _ Hv Hdv) => [Hda [Hwta Htyv]]. exact: (well_typed_eexp_of_atom Hwta).
+      + done.
+    - move=> op e1 IH1 e2 IH2. rewrite are_defined_union => /andP [Hdef1 Hdef2].
+      move/andP=> [Hwt1 Hwt2]. rewrite (IH1 Hdef1 Hwt1) (IH2 Hdef2 Hwt2). reflexivity.
+  Qed.
+
+  Lemma subst_eexp_well_formed E m e :
+    weak_consistent_type m E ->
+    well_formed_eexp E e ->
+    well_formed_eexp E (subst_eexp m e).
+  Proof.
+    move=> Hco. rewrite /well_formed_eexp. move/andP => [Hdef Hwt].
+    rewrite (subst_eexp_are_defined Hco Hdef) (subst_eexp_well_typed Hco Hdef Hwt).
+    reflexivity.
+  Qed.
+
+  Lemma subst_rexp_are_defined E m e :
+    weak_consistent_type m E ->
+    are_defined (vars_rexp e) E ->
+    are_defined (vars_rexp (subst_rexp m e)) E.
+  Proof.
+    move => Hco. elim: e => //=.
+    - move=> v. rewrite are_defined_singleton /= => Hdv.
+      case Hv: (SSAVM.find v m).
+      + move: (Hco _ _ Hv Hdv) => [Hda [Hwta Htyv]]. rewrite vars_rexp_of_atom.
+        exact: Hda.
+      + simpl. rewrite are_defined_singleton. exact: Hdv.
+    - move=> w op e1 IH1 e2 IH2. rewrite 2!are_defined_union. move/andP => [Hdef1 Hdef2].
+      rewrite (IH1 Hdef1) (IH2 Hdef2). reflexivity.
+  Qed.
+
+  Lemma subst_rexp_well_typed E m e :
+    weak_consistent_type m E ->
+    are_defined (vars_rexp e) E ->
+    well_typed_rexp E e ->
+    well_typed_rexp E (subst_rexp m e).
+  Proof.
+    move => Hco. elim: e => //=.
+    - move=> v. rewrite are_defined_singleton. move => Hdv Hsv. case Hv: (SSAVM.find v m).
+      + move: (Hco _ _ Hv Hdv) => [Hda [Hwta Htyv]]. exact: (well_typed_rexp_of_atom Hwta).
+      + simpl. exact: Hsv.
+    - move=> w op e IH Hdef H. caseb H. move=> Hw Hwt Hse.
+      rewrite Hw (IH Hdef Hwt) (weak_consistent_type_size_of_subst_rexp Hco) /=; first assumption.
+      rewrite /well_formed_rexp. by rewrite Hdef Hwt.
+    - move=> w op e1 IH1 e2 IH2. rewrite are_defined_union => /andP [Hdef1 Hdef2].
+      move=> H. caseb H. move=> Hw Hwt1 Hs1 Hwt2 Hs2.
+      have Hwf1: well_formed_rexp E e1 by rewrite /well_formed_rexp Hdef1 Hwt1.
+      have Hwf2: well_formed_rexp E e2 by rewrite /well_formed_rexp Hdef2 Hwt2.
+      rewrite (weak_consistent_type_size_of_subst_rexp Hco Hwf1)
+              (weak_consistent_type_size_of_subst_rexp Hco Hwf2).
+      rewrite (IH1 Hdef1 Hwt1) (IH2 Hdef2 Hwt2) Hw Hs1 Hs2. reflexivity.
+    - move=> w e IH n Hdef. move=> H; caseb H. move=> Hw Hwt Hs.
+      have Hwf: well_formed_rexp E e by rewrite /well_formed_rexp Hdef Hwt.
+      rewrite (weak_consistent_type_size_of_subst_rexp Hco Hwf).
+      rewrite (IH Hdef Hwt) Hw Hs. reflexivity.
+    - move=> w e IH n Hdef. move=> H; caseb H. move=> Hw Hwt Hs.
+      have Hwf: well_formed_rexp E e by rewrite /well_formed_rexp Hdef Hwt.
+      rewrite (weak_consistent_type_size_of_subst_rexp Hco Hwf).
+      rewrite (IH Hdef Hwt) Hw Hs. reflexivity.
+  Qed.
+
+  Lemma subst_rexp_well_formed E m e :
+    weak_consistent_type m E ->
+    well_formed_rexp E e ->
+    well_formed_rexp E (subst_rexp m e).
+  Proof.
+    move=> Hco. rewrite /well_formed_rexp. move/andP => [Hdef Hwt].
+    rewrite (subst_rexp_are_defined Hco Hdef) (subst_rexp_well_typed Hco Hdef Hwt).
+    reflexivity.
+  Qed.
+
+  Lemma subst_eexps_are_defined E m es :
+    weak_consistent_type m E ->
+    are_defined (vars_eexps es) E ->
+    are_defined (vars_eexps (subst_eexps m es)) E.
+  Proof.
+    move=> Hco. elim: es => [| e es IH] //=.
+    rewrite subst_eexps_cons /= 2!are_defined_union => /andP [He Hes].
+    rewrite (subst_eexp_are_defined Hco He) (IH Hes). reflexivity.
+  Qed.
+
+  Lemma subst_eexps_well_typed E m es :
+    weak_consistent_type m E ->
+    are_defined (vars_eexps es) E ->
+    well_typed_eexps E es ->
+    well_typed_eexps E (subst_eexps m es).
+  Proof.
+    move=> Hco. elim: es => [| e es IH] //=.
+    rewrite subst_eexps_cons /= are_defined_union => /andP [He Hes].
+    move/andP => [Hwfe Hwfes]. rewrite (subst_eexp_well_typed Hco He Hwfe) (IH Hes Hwfes).
+    reflexivity.
+  Qed.
+
+  Lemma subst_eexps_well_formed E m es :
+    weak_consistent_type m E ->
+    well_formed_eexps E es ->
+    well_formed_eexps E (subst_eexps m es).
+  Proof.
+    move=> Hco. elim: es => [| e es IH] //=. move/andP => [Hwfe Hwfes].
+    rewrite subst_eexps_cons /=. rewrite (subst_eexp_well_formed Hco Hwfe) (IH Hwfes).
+    reflexivity.
+  Qed.
+
+  Lemma subst_ebexp_are_defined E m e :
+    weak_consistent_type m E ->
+    are_defined (vars_ebexp e) E ->
+    are_defined (vars_ebexp (subst_ebexp m e)) E.
+  Proof.
+    move => Hco. elim: e => //=.
+    - move=> e1 e2. rewrite 2!are_defined_union => /andP [Hdef1 Hdef2].
+      rewrite (subst_eexp_are_defined Hco Hdef1) (subst_eexp_are_defined Hco Hdef2).
+      reflexivity.
+    - move=> e1 e2 ms. rewrite !are_defined_union => H; caseb H.
+      move=> Hdef1 Hdef2 Hdefms.
+      rewrite (subst_eexp_are_defined Hco Hdef1) (subst_eexp_are_defined Hco Hdef2)
+              (subst_eexps_are_defined Hco Hdefms). reflexivity.
+    - move=> e1 IH1 e2 IH2. rewrite 2!are_defined_union => /andP [Hdef1 Hdef2].
+      rewrite (IH1 Hdef1) (IH2 Hdef2). reflexivity.
+  Qed.
+
+  Lemma subst_ebexp_well_typed E m e :
+    weak_consistent_type m E ->
+    are_defined (vars_ebexp e) E ->
+    well_typed_ebexp E e ->
+    well_typed_ebexp E (subst_ebexp m e).
+  Proof.
+    move => Hco. elim: e => //=.
+    - move=> e1 e2. rewrite are_defined_union => /andP [Hdef1 Hdef2].
+      move/andP => [Hwt1 Hwt2]. rewrite (subst_eexp_well_typed Hco Hdef1 Hwt1)
+                                        (subst_eexp_well_typed Hco Hdef2 Hwt2).
+      reflexivity.
+    - move=> e1 e2 ms. rewrite !are_defined_union => H; caseb H.
+      move=> Hdef1 Hdef2 Hdefms. move=> H; caseb H. move=> Hwt1 Hwt2 Hwtms.
+      rewrite (subst_eexp_well_typed Hco Hdef1 Hwt1) (subst_eexp_well_typed Hco Hdef2 Hwt2)
+              (subst_eexps_well_typed Hco Hdefms Hwtms). reflexivity.
+    - move=> e1 IH1 e2 IH2. rewrite are_defined_union => /andP [Hdef1 Hdef2].
+      move/andP => [Hwt1 Hwt2]. rewrite (IH1 Hdef1 Hwt1) (IH2 Hdef2 Hwt2). reflexivity.
+  Qed.
+
+  Lemma subst_ebexp_well_formed E m e :
+    weak_consistent_type m E ->
+    well_formed_ebexp E e ->
+    well_formed_ebexp E (subst_ebexp m e).
+  Proof.
+    move=> Hco. rewrite /well_formed_ebexp. move/andP => [Hdef Hwt].
+    rewrite (subst_ebexp_are_defined Hco Hdef) (subst_ebexp_well_typed Hco Hdef Hwt).
+    reflexivity.
+  Qed.
+
+  Lemma subst_rbexp_are_defined E m e :
+    weak_consistent_type m E ->
+    are_defined (vars_rbexp e) E ->
+    are_defined (vars_rbexp (subst_rbexp m e)) E.
+  Proof.
+    move => Hco. elim: e => //=.
+    - move=> w e1 e2. rewrite 2!are_defined_union => /andP [Hdef1 Hdef2].
+      rewrite (subst_rexp_are_defined Hco Hdef1) (subst_rexp_are_defined Hco Hdef2).
+      reflexivity.
+    - move=> w op e1 e2. rewrite 2!are_defined_union => /andP [Hdef1 Hdef2].
+      rewrite (subst_rexp_are_defined Hco Hdef1) (subst_rexp_are_defined Hco Hdef2).
+      reflexivity.
+    - move=> e1 IH1 e2 IH2. rewrite 2!are_defined_union => /andP [Hdef1 Hdef2].
+      rewrite (IH1 Hdef1) (IH2 Hdef2). reflexivity.
+    - move=> e1 IH1 e2 IH2. rewrite 2!are_defined_union => /andP [Hdef1 Hdef2].
+      rewrite (IH1 Hdef1) (IH2 Hdef2). reflexivity.
+  Qed.
+
+  Lemma subst_rbexp_well_typed E m e :
+    weak_consistent_type m E ->
+    are_defined (vars_rbexp e) E ->
+    well_typed_rbexp E e ->
+    well_typed_rbexp E (subst_rbexp m e).
+  Proof.
+    move => Hco. elim: e => //=.
+    - move=> w e1 e2. rewrite are_defined_union => H1 H2; caseb H2; caseb H1.
+      move=> Hdef1 Hdef2 Hw Hwt1 Hs1 Hwt2 Hs2.
+      rewrite (subst_rexp_well_typed Hco Hdef1 Hwt1) (subst_rexp_well_typed Hco Hdef2 Hwt2).
+      have Hwf1: well_formed_rexp E e1 by rewrite /well_formed_rexp Hdef1 Hwt1.
+      have Hwf2: well_formed_rexp E e2 by rewrite /well_formed_rexp Hdef2 Hwt2.
+      rewrite (weak_consistent_type_size_of_subst_rexp Hco Hwf1)
+              (weak_consistent_type_size_of_subst_rexp Hco Hwf2).
+      rewrite Hw Hs1 Hs2. reflexivity.
+    - move=> w op e1 e2. rewrite are_defined_union => H1 H2; caseb H2; caseb H1.
+      move=> Hdef1 Hdef2 Hw Hwt1 Hs1 Hwt2 Hs2.
+      rewrite (subst_rexp_well_typed Hco Hdef1 Hwt1) (subst_rexp_well_typed Hco Hdef2 Hwt2).
+      have Hwf1: well_formed_rexp E e1 by rewrite /well_formed_rexp Hdef1 Hwt1.
+      have Hwf2: well_formed_rexp E e2 by rewrite /well_formed_rexp Hdef2 Hwt2.
+      rewrite (weak_consistent_type_size_of_subst_rexp Hco Hwf1)
+              (weak_consistent_type_size_of_subst_rexp Hco Hwf2).
+      rewrite Hw Hs1 Hs2. reflexivity.
+    - move=> e1 IH1 e2 IH2. rewrite are_defined_union => /andP [Hdef1 Hdef2] /andP [Hwt1 Hwt2].
+      rewrite (IH1 Hdef1 Hwt1) (IH2 Hdef2 Hwt2). reflexivity.
+    - move=> e1 IH1 e2 IH2. rewrite are_defined_union => /andP [Hdef1 Hdef2] /andP [Hwt1 Hwt2].
+      rewrite (IH1 Hdef1 Hwt1) (IH2 Hdef2 Hwt2). reflexivity.
+  Qed.
+
+  Lemma subst_rbexp_well_formed E m e :
+    weak_consistent_type m E ->
+    well_formed_rbexp E e ->
+    well_formed_rbexp E (subst_rbexp m e).
+  Proof.
+    move=> Hco. rewrite /well_formed_rbexp. move/andP => [Hdef Hwt].
+    rewrite (subst_rbexp_are_defined Hco Hdef) (subst_rbexp_well_typed Hco Hdef Hwt).
+    reflexivity.
+  Qed.
+
+  Lemma subst_bexp_are_defined E m e :
+    weak_consistent_type m E ->
+    are_defined (vars_bexp e) E ->
+    are_defined (vars_bexp (subst_bexp m e)) E.
+  Proof.
+    move=> Hco. case: e => [e r]. rewrite /vars_bexp /subst_bexp /=.
+    rewrite 2!are_defined_union => /andP [Hdefe Hdefr].
+    rewrite (subst_ebexp_are_defined Hco Hdefe) (subst_rbexp_are_defined Hco Hdefr).
+    reflexivity.
+  Qed.
+
+  Lemma subst_bexp_well_typed E m e :
+    weak_consistent_type m E ->
+    are_defined (vars_bexp e) E ->
+    well_typed_bexp E e ->
+    well_typed_bexp E (subst_bexp m e).
+  Proof.
+    move=> Hco. case: e => [e r]. rewrite /subst_bexp /vars_bexp /well_typed_bexp /=.
+    rewrite are_defined_union => /andP [Hdefe Hdefr] /andP [Hwte Hwtr].
+    rewrite (subst_ebexp_well_typed Hco Hdefe Hwte)
+            (subst_rbexp_well_typed Hco Hdefr Hwtr). reflexivity.
+  Qed.
+
+  Lemma subst_bexp_well_formed E m e :
+    weak_consistent_type m E ->
+    well_formed_bexp E e ->
+    well_formed_bexp E (subst_bexp m e).
+  Proof.
+    move=> Hco. case: e => [e r]. rewrite /subst_bexp /= 2!well_formed_bexp_split /=.
+    move/andP => [Hwfe Hwfr]. rewrite (subst_ebexp_well_formed Hco Hwfe)
+                                      (subst_rbexp_well_formed Hco Hwfr). reflexivity.
+  Qed.
+
+  Lemma subst_instr_well_formed E m i :
+    weak_consistent_type m E ->
+    well_formed_instr E i ->
+    well_formed_instr E (subst_instr m i).
+  Proof.
+    move=> Hco.
+    (case: i => //=); (rewrite /well_formed_instr /=); intros;
+      by repeat match goal with
+                | |- is_true true => reflexivity
+                | H : is_true ?e |- context [?e] => rewrite H /=
+                | H : is_true (_ && _) |- _ =>
+                    caseb H; intros
+                | Hco : weak_consistent_type ?m ?E,
+                    Hda : is_true (are_defined (vars_atom ?a) ?E)
+                  |- context [are_defined (vars_atom (subst_atom ?m ?a)) ?E] =>
+                    rewrite (weak_consistent_type_are_defined_atom Hco Hda) /=
+                | Hco : weak_consistent_type ?m ?E,
+                    Hda : is_true (are_defined (vars_atom ?a) ?E),
+                      Hwt : is_true (well_typed_atom ?E ?a)
+                  |- context [well_typed_atom ?E (subst_atom ?m ?a)] =>
+                    rewrite (weak_consistent_type_well_typed_atom Hco Hda Hwt) /=
+                | Hco : weak_consistent_type ?m ?E,
+                    Hda : is_true (are_defined (vars_atom ?a) ?E)
+                  |- context [atyp (subst_atom ?m ?a) ?E] =>
+                    rewrite (weak_consistent_type_atyp Hco Hda) /=
+                | Hco : weak_consistent_type ?m ?E,
+                    Hda : is_true (are_defined (vars_atom ?a) ?E)
+                  |- context [asize (subst_atom ?m ?a) ?E] =>
+                    rewrite (weak_consistent_type_asize Hco Hda) /=
+                | Hco : weak_consistent_type ?m ?E,
+                    Hdef : is_true (are_defined (vars_bexp ?b) ?E)
+                  |- context [are_defined (vars_bexp (subst_bexp ?m ?b)) ?E] =>
+                    rewrite (subst_bexp_are_defined Hco Hdef) /=
+                | Hco : weak_consistent_type ?m ?E,
+                    Hdef : is_true (are_defined (vars_bexp ?b) ?E),
+                      Hwt : is_true (well_typed_bexp ?E ?b)
+                  |- context [well_typed_bexp E (subst_bexp ?m ?b)] =>
+                    rewrite (subst_bexp_well_typed Hco Hdef Hwt) /=
+                end.
+  Qed.
+
+  Lemma subst_program_well_formed E m p :
+    weak_consistent_type_chain E m p ->
+    well_formed_program E p ->
+    well_formed_program E (subst_program m p).
+  Proof.
+    elim: p E m => [| i p IH] E m //=. move=> [Hco Hsucc] /andP [Hwfi Hwfp].
+    rewrite subst_program_cons /=. rewrite (subst_instr_well_formed Hco Hwfi) /=.
+    rewrite (weak_consistent_type_instr_succ_typenv Hco Hwfi).
+    exact: (IH _ _ Hsucc Hwfp).
+  Qed.
+
+  Lemma lvs_subst_instr m i :
+    SSAVS.Equal (lvs_instr (subst_instr m i)) (lvs_instr i).
+  Proof. by case: i => //=. Qed.
+
+  Lemma lvs_subst_program m p :
+    SSAVS.Equal (lvs_program (subst_program m p)) (lvs_program p).
+  Proof.
+    elim: p => [| i p IH] //=. rewrite subst_program_cons /=.
+    rewrite lvs_subst_instr IH. reflexivity.
+  Qed.
+
+  Lemma subst_program_single_assignment E m p :
+    well_formed_ssa_program E p ->
+    weak_consistent_type_chain E m p ->
+    ssa_single_assignment (subst_program m p).
+  Proof.
+    elim: p m E => [| i p IH] m E //=. move=> Hwf [Hcoi Hcop].
+    rewrite subst_program_cons /=. rewrite (IH _ _ (well_formed_ssa_tl Hwf) Hcop) andbT.
+    rewrite lvs_subst_instr. rewrite ssa_unchanged_program_disjoint_lvs.
+    rewrite lvs_subst_program. rewrite -ssa_unchanged_program_disjoint_lvs.
+    apply: (ssa_unchanged_program_subset _ (lvs_instr_subset _)).
+    exact: (well_formed_ssa_vars_unchanged_hd Hwf).
+  Qed.
+
+  Lemma rewrite_mov_well_formed_ssa s :
+    well_formed_ssa_spec s ->
+    well_formed_ssa_spec (rewrite_mov s).
+  Proof.
+    case: s => E f p g. rewrite /well_formed_ssa_spec /=.
+    rewrite /well_formed_spec /rewrite_mov /subst_map_spec /=.
+    move=> Hwf. caseb Hwf. move=> Hwff Hwfp Hwfg HunEp Hssap.
+    have Hwfssap: well_formed_ssa_program E p.
+    { rewrite /well_formed_ssa_program. by rewrite Hwfp HunEp Hssap. }
+    rewrite (subst_map_program_succ_typenv Hwfssap).
+    move: (subst_map_program_weak_consistent_type_init Hwfssap) => Hcowty.
+    move: (subst_map_program_consistent_type Hwfssap) => Hcoty.
+    move: (subst_map_program_weak_consistent_type_chain Hwfssap) => Hcowcty.
+    have Hdisjfm: VSLemmas.disjoint (vars_bexp f) (TEKS.key_set (subst_map_program p)).
+    { apply: (VSLemmas.disjoint_subset_r _ (subst_map_program_keys_subset p)).
+      rewrite -ssa_unchanged_program_disjoint_lvs. apply: (ssa_unchanged_program_subset HunEp).
+      exact: (well_formed_bexp_vars_subset Hwff). }
+    (* f *)
+    rewrite (weak_consistent_type_disjoint_well_formed_bexp Hcowty Hdisjfm) Hwff /=.
+    (* p *)
+    rewrite (subst_program_well_formed Hcowcty Hwfp) /=.
+    (* g *)
+    rewrite (subst_bexp_well_formed (consistent_type_weak Hcoty) Hwfg) /=.
+    (* env unchanged *)
+    rewrite ssa_unchanged_program_disjoint_lvs. rewrite lvs_subst_program.
+    rewrite -ssa_unchanged_program_disjoint_lvs. rewrite HunEp /=.
+    (* single assignment *)
+    exact: (subst_program_single_assignment Hwfssap Hcowcty).
+  Qed.
+
+End RewriteMov.
 
 
 Section Extra.
@@ -505,42 +3068,6 @@ Section Extra.
   Qed.
 
 End Extra.
-
-
-(* Rewrite mov statements in AST level - to be implemented for optimization *)
-
-Section RewriteMov.
-
-  Import SSA.
-
-  Definition rewrite_mov (s : spec) : spec := s.
-
-  Lemma rewrite_mov_vars s : SSAVS.Equal (vars_spec (rewrite_mov s)) (vars_spec s).
-  Proof. reflexivity. Qed.
-
-  Lemma rewrite_mov_sound s :
-    well_formed_ssa_spec s ->
-    valid_spec (rewrite_mov s) -> valid_spec s.
-  Proof. move=> _. by apply. Qed.
-
-  Lemma rewrite_mov_complete s :
-    well_formed_ssa_spec s ->
-    valid_spec s -> valid_spec (rewrite_mov s).
-  Proof. move=> _. by apply. Qed.
-
-  Lemma rewrite_mov_well_formed_ssa s :
-    well_formed_ssa_spec s ->
-    well_formed_ssa_spec (rewrite_mov s).
-  Proof. by apply. Qed.
-
-  Lemma rewrite_mov_succ_typenv s :
-    well_formed_ssa_spec s ->
-    SSATE.Equal
-             (program_succ_typenv (sprog (rewrite_mov s)) (sinputs (rewrite_mov s)))
-             (program_succ_typenv (sprog s) (sinputs s)).
-  Proof. reflexivity. Qed.
-
-End RewriteMov.
 
 
 (* Convert SSAFull without Iassert and Icut statements to SSA *)
